NuSys.thy
@@ -3,10 +3,10 @@
 theory NuSys
   imports NuPrime NuLLReps
   keywords
-    "proc" "proc'" "rec_proc" :: thy_goal_stmt
+    "proc" "proc'" (* "rec_proc" *) :: thy_goal_stmt
   and "as" "\<rightarrow>" "\<longmapsto>" "\<leftarrow>" "^" "^*" "cast" "requires" "\<Longleftarrow>" "\<Longleftarrow>'" "$" "var" "always" :: quasi_command
-  and "\<bullet>" "affirm" "\<nu>have" "\<nu>obtain" "\<nu>choose" "\<nu>choose2" "\<medium_left_bracket>" "\<medium_right_bracket>" "\<Longrightarrow>" "drop_fact" "\<nu>debug" "\<nu>debug'"
-          "\<nu>note" "\<nu>choose_quick" :: prf_decl % "proof"
+  and "\<bullet>" "affirm" "\<nu>have" (* "\<nu>obtain" "\<nu>choose" "\<nu>choose2" *) "\<medium_left_bracket>" "\<medium_right_bracket>" "\<Longrightarrow>" "drop_fact" "\<nu>debug" "\<nu>debug'"
+          "\<nu>note" (* "\<nu>choose_quick" *) :: prf_decl % "proof"
   and "\<nu>processor" "\<nu>processor_resolver" "\<nu>exty_simproc" :: thy_decl % "ML"
   and "\<nu>overloads" "\<nu>cast_overloads" :: thy_decl
   and "finish" :: "qed" % "proof"
@@ -28,6 +28,46 @@ lemma [final_proc_rewrite2]: "\<^bold>p\<^bold>r\<^bold>e\<^bold>m\<^bold>i\<^bo
 definition  FailedPremise :: "bool \<Rightarrow> bool" where "FailedPremise \<equiv> Premise"
 lemma FailedPremise_I: "\<^bold>p\<^bold>r\<^bold>e\<^bold>m\<^bold>i\<^bold>s\<^bold>e P \<Longrightarrow> FailedPremise P" unfolding FailedPremise_def .
 lemma FailedPremise_D: "FailedPremise P \<Longrightarrow> \<^bold>p\<^bold>r\<^bold>e\<^bold>m\<^bold>i\<^bold>s\<^bold>e P" unfolding FailedPremise_def .
+
+ML_file NuHelp.ML
+
+subsection \<open>Syntax Helper\<close>
+
+ML \<open>
+fun parse_typing_ty (Type (\<^type_name>\<open>typing\<close>, [a,b])) = (b, a --> b --> \<^typ>\<open>bool\<close>)
+  | parse_typing_ty dummyT = (dummyT, dummyT)
+  | parse_typing_ty ty = raise TYPE ("should be a typing type", [ty], [])
+
+fun parse_typing (Free (name, ty)) =
+    Const (\<^const_syntax>\<open>typing\<close>, ty) $ Free (name^"\<^sub>x", fst (parse_typing_ty ty))
+        $ Free (name^"\<^sub>t\<^sub>y", snd (parse_typing_ty ty))
+  | parse_typing (Var ((name,ind), ty)) =
+    Const (\<^const_syntax>\<open>typing\<close>, ty) $ Var ((name^"\<^sub>x",ind), fst (parse_typing_ty ty))
+        $ Var ((name^"\<^sub>t\<^sub>y", ind), snd (parse_typing_ty ty))
+  | parse_typing (Const (\<^syntax_const>\<open>_constrain\<close>, ty) $ tm $ (Const (\<^type_syntax>\<open>typing\<close>, _) $ tya $ tyb)) =
+      let val (const $ tmx $ tmty) = parse_typing tm
+      in const $ (Const (\<^syntax_const>\<open>_constrain\<close>, ty) $ tmx $ tyb)
+        $ (Const (\<^syntax_const>\<open>_constrain\<close>, ty) $ tmty $ (Const (\<^type_syntax>\<open>\<nu>\<close>, dummyT) $ tya $ tyb)) end
+  | parse_typing (Const (\<^syntax_const>\<open>_constrain\<close>, ty) $ tm $ markup) =
+      let val (const $ tmx $ tmty) = parse_typing tm
+      in const $ (Const (\<^syntax_const>\<open>_constrain\<close>, ty) $ tmx $ markup)
+        $ (Const (\<^syntax_const>\<open>_constrain\<close>, ty) $ tmty $ markup) end
+  | parse_typing (tm as Const (\<^const_syntax>\<open>typing\<close>, _) $ _ $ _) = tm
+  | parse_typing tm = raise TERM ("should be a NuPrime.typing term", [@{print} tm])
+
+fun parse_typing_x tm = (case parse_typing tm of _ $ x $ _ => x)
+fun parse_typing_ty tm = (case parse_typing tm of _ $ _ $ ty => ty)
+\<close>
+
+syntax "_\<nu>typing" :: " logic \<Rightarrow> logic "
+  "_\<nu>typing_x" :: " logic \<Rightarrow> logic "
+  "_\<nu>typing_ty" :: " logic \<Rightarrow> logic "
+parse_translation \<open>[
+  (\<^syntax_const>\<open>_\<nu>typing\<close>, (fn _ => fn [tm] => parse_typing tm)),
+  (\<^syntax_const>\<open>_\<nu>typing_x\<close>, (fn _ => fn [tm] => parse_typing_x tm)),
+  (\<^syntax_const>\<open>_\<nu>typing_ty\<close>, (fn _ => fn [tm] => parse_typing_ty tm))
+]\<close>
+
 
 section \<open>Mechanisms - I\<close>
 
@@ -72,7 +112,7 @@ lemma cast_id[\<nu>intro0]: "\<^bold>c\<^bold>a\<^bold>s\<^bold>t A \<longmapsto
 lemma cast_dual_id[\<nu>intro0]: "\<^bold>c\<^bold>a\<^bold>s\<^bold>t A \<longmapsto> A \<^bold>d\<^bold>u\<^bold>a\<^bold>l B \<longmapsto> B" unfolding CastDual_def  by (simp add: cast_id)
 
 lemma "=_\<nu>cast": "\<^bold>p\<^bold>a\<^bold>r\<^bold>a\<^bold>m x' \<Longrightarrow> \<^bold>p\<^bold>r\<^bold>e\<^bold>m\<^bold>i\<^bold>s\<^bold>e x = x' \<Longrightarrow> \<^bold>c\<^bold>a\<^bold>s\<^bold>t x \<tycolon> N \<longmapsto> x' \<tycolon> N" unfolding Cast_def by auto
-lemma [\<nu>intro']: "\<^bold>p\<^bold>r\<^bold>e\<^bold>m\<^bold>i\<^bold>s\<^bold>e N = N' \<Longrightarrow> \<^bold>p\<^bold>r\<^bold>e\<^bold>m\<^bold>i\<^bold>s\<^bold>e x = x' \<Longrightarrow> \<^bold>c\<^bold>a\<^bold>s\<^bold>t \<tort_lbrace>x \<tycolon> N\<tort_rbrace> \<longmapsto> \<tort_lbrace>x' \<tycolon> N'\<tort_rbrace>" unfolding Cast_def Premise_def by simp
+lemma [\<nu>intro']: "\<^bold>p\<^bold>r\<^bold>e\<^bold>m\<^bold>i\<^bold>s\<^bold>e N = N' \<Longrightarrow> \<^bold>p\<^bold>r\<^bold>e\<^bold>m\<^bold>i\<^bold>s\<^bold>e x = x' \<Longrightarrow> \<^bold>c\<^bold>a\<^bold>s\<^bold>t x \<tycolon> N \<longmapsto> x' \<tycolon> N'" unfolding Cast_def Premise_def by simp
 lemma [\<nu>intro0]: "\<^bold>p\<^bold>r\<^bold>e\<^bold>m\<^bold>i\<^bold>s\<^bold>e x = x" unfolding Premise_def by simp
 
 lemma cast_trans: "\<^bold>c\<^bold>a\<^bold>s\<^bold>t A \<longmapsto> B \<^bold>w\<^bold>i\<^bold>t\<^bold>h P \<Longrightarrow> \<^bold>c\<^bold>a\<^bold>s\<^bold>t B \<longmapsto> C \<^bold>w\<^bold>i\<^bold>t\<^bold>h Q \<Longrightarrow> \<^bold>c\<^bold>a\<^bold>s\<^bold>t A \<longmapsto> C \<^bold>w\<^bold>i\<^bold>t\<^bold>h P \<and> Q"
@@ -87,23 +127,23 @@ subsection \<open>Separation Conjecture\<close>
 definition disjoint :: " 'a set \<Rightarrow> 'a set \<Rightarrow> bool " (infixl "\<perpendicular>" 60) where "disjoint A B \<longleftrightarrow> (A \<inter> B = {})"
 lemma disjoint_rewL: "A \<perpendicular> B \<longleftrightarrow> (\<forall>x. x \<in> A \<longrightarrow> x \<notin> B)" unfolding disjoint_def by auto
 lemma disjoint_rewR: "A \<perpendicular> B \<longleftrightarrow> (\<forall>x. x \<in> B \<longrightarrow> x \<notin> A)" unfolding disjoint_def by auto
+lemma [elim]: "A \<perpendicular> B \<Longrightarrow> ((\<And>x. x \<in> A \<Longrightarrow> x \<in> B \<Longrightarrow> False) \<Longrightarrow> C) \<Longrightarrow> C" unfolding disjoint_def by auto
 
 lemma [iff]: "{} \<perpendicular> S" and [iff]: "S \<perpendicular> {}" unfolding disjoint_def by auto
 
 definition Separation :: " (heap, 'a) \<nu> \<Rightarrow> (heap, 'b) \<nu> \<Rightarrow> (heap, 'a \<times> 'b) \<nu>" (infixr "\<^emph>" 70)
-  where "A \<^emph> B = (\<lambda>h (a,b). (\<exists>h1 h2. h = h1 ++ h2 \<and> dom h1 \<perpendicular> dom h2 \<and> (h1 \<nuLinkL> A \<nuLinkR> a) \<and> (h2 \<nuLinkL> B \<nuLinkR> b)))"
+  where "A \<^emph> B = (\<lambda>h (a,b). (\<exists>h2 h1. h = h2 ++ h1 \<and> dom h2 \<perpendicular> dom h1 \<and> (h1 \<nuLinkL> A \<nuLinkR> a) \<and> (h2 \<nuLinkL> B \<nuLinkR> b)))"
 
-lemma [iff]: "h \<nuLinkL> A \<^emph> B \<nuLinkR> (a,b) \<longleftrightarrow>
-  (\<exists>h1 h2. h = h1 ++ h2 \<and> dom h1 \<perpendicular> dom h2 \<and> (h1 \<nuLinkL> A \<nuLinkR> a) \<and> (h2 \<nuLinkL> B \<nuLinkR> b))"
+lemma Separation_exp[iff]: "h \<nuLinkL> A \<^emph> B \<nuLinkR> (a,b) \<longleftrightarrow>
+  (\<exists>h2 h1. h = h2 ++ h1 \<and> dom h2 \<perpendicular> dom h1 \<and> (h1 \<nuLinkL> A \<nuLinkR> a) \<and> (h2 \<nuLinkL> B \<nuLinkR> b))"
   unfolding Separation_def Refining_ex by simp
 
 definition Heap_Delimiter :: "(heap,'ax) \<nu> \<Rightarrow> (heap,'bx) \<nu> \<Rightarrow> (heap, 'ax \<times> 'bx) \<nu>" (infixr "<heap-sep>" 70)
   where "A <heap-sep> B = A \<^emph> B"
-abbreviation Heap_Delimiter_sugar :: " (heap, 'ax) typing \<Rightarrow> (heap, 'bx) typing \<Rightarrow> (heap, 'bx \<times> 'ax) typing " ( "_/ \<heavy_asterisk> _" [14,15] 14)
-  where "(A \<heavy_asterisk> B) \<equiv> (typing_img B, typing_img A) \<tycolon> (typing_nu B <heap-sep> typing_nu A)"
+consts Heap_Delimiter_sugar :: " 'just \<Rightarrow> 'a \<Rightarrow> 'sugar " ( "_/ \<heavy_asterisk> _" [14,15] 14) \<comment> \<open>It is left associative!\<close>
 
-lemma [simp]: " (a \<tycolon> A \<heavy_asterisk> b \<tycolon> B) = ((b,a) \<tycolon> (B <heap-sep> A)) " by auto
 translations " (a \<tycolon> A) \<heavy_asterisk> (b \<tycolon> B) " \<rightleftharpoons> " (CONST Pair b a) \<tycolon> (B <heap-sep> A) "
+  " A \<heavy_asterisk> B " => " (CONST Pair (_\<nu>typing_x B) (_\<nu>typing_x A)) \<tycolon> ((_\<nu>typing_ty B) <heap-sep> (_\<nu>typing_ty A)) "
 
 lemma [cong]: "\<tort_lbrace> a \<tycolon> A \<tort_rbrace> \<equiv> \<tort_lbrace>a' \<tycolon> A'\<tort_rbrace> \<Longrightarrow> \<tort_lbrace> b \<tycolon> B \<tort_rbrace> \<equiv> \<tort_lbrace>b' \<tycolon> B'\<tort_rbrace> \<Longrightarrow> \<tort_lbrace> a \<tycolon> A \<heavy_asterisk> b \<tycolon> B \<tort_rbrace> \<equiv> \<tort_lbrace> a' \<tycolon> A' \<heavy_asterisk> b' \<tycolon> B' \<tort_rbrace>"
   unfolding atomize_eq unfolding Heap_Delimiter_def by auto
@@ -136,13 +176,24 @@ lemma heap_split_by_set: "P (h |` S) (h |` (- S)) \<Longrightarrow> \<exists>h1 
 lemma heap_split_by_addr_set: "P (h |` (MemAddress ` S)) (h |` (- (MemAddress ` S))) \<Longrightarrow> \<exists>h1 h2. h = h1 ++ h2 \<and> dom h1 \<perpendicular> dom h2 \<and> P h1 h2"
   using heap_split_by_set .
 
-lemma Separation_comm: " \<tort_lbrace> a \<tycolon> A \<heavy_asterisk> b \<tycolon> B\<tort_rbrace> = \<tort_lbrace>b \<tycolon> B \<heavy_asterisk> a \<tycolon> A\<tort_rbrace>" unfolding Heap_Delimiter_def
+
+
+
+definition SeparationSet :: " heap set \<Rightarrow> heap set \<Rightarrow> heap set" (infixr "<sep-set>" 70)
+  where "A <sep-set> B = {h. (\<exists>h1 h2. h = h1 ++ h2 \<and> dom h1 \<perpendicular> dom h2 \<and> h1 \<in> A \<and> h2 \<in> B)}"
+lemma SepNu_2_SepSet: "\<tort_lbrace> h1 \<tycolon> H1 \<heavy_asterisk> h2 \<tycolon> H2 \<tort_rbrace> = \<tort_lbrace> h1 \<tycolon> H1 \<tort_rbrace> <sep-set> \<tort_lbrace> h2 \<tycolon> H2 \<tort_rbrace>"
+  unfolding SeparationSet_def Heap_Delimiter_def by auto
+
+lemma SeparationSet_comm: " A <sep-set> B = B <sep-set> A" unfolding SeparationSet_def
   by (auto 4 4 simp add: disjoint_def inf_commute dest: map_add_comm )
- 
-lemma Separation_assoc: "\<tort_lbrace> a \<tycolon> A \<heavy_asterisk> (b \<tycolon> B \<heavy_asterisk> c \<tycolon> C)\<tort_rbrace> = \<tort_lbrace>a \<tycolon> A \<heavy_asterisk> b \<tycolon> B \<heavy_asterisk> c \<tycolon> C\<tort_rbrace>"
-  unfolding Heap_Delimiter_def
-  by (auto simp add: disjoint_def) 
-    (metis (no_types, lifting) Un_empty dom_map_add inf_sup_distrib1 inf_sup_distrib2 map_add_assoc)+
+lemma Separation_comm: " \<tort_lbrace> A \<heavy_asterisk> B\<tort_rbrace> = \<tort_lbrace> B \<heavy_asterisk> A\<tort_rbrace>"
+  unfolding SepNu_2_SepSet using SeparationSet_comm by fast
+
+lemma SeparationSet_assoc: " (A <sep-set> B) <sep-set> C = A <sep-set> B <sep-set> C"
+  unfolding SeparationSet_def
+  by (auto simp add: disjoint_def) (metis (no_types, lifting) Un_empty dom_map_add inf_sup_distrib1 inf_sup_distrib2 map_add_assoc)+
+lemma Separation_assoc: "\<tort_lbrace> A \<heavy_asterisk> (B \<heavy_asterisk> C)\<tort_rbrace> = \<tort_lbrace> A \<heavy_asterisk> B \<heavy_asterisk> C\<tort_rbrace>"
+  unfolding SepNu_2_SepSet using SeparationSet_assoc by fast
 
 (* lemma NonSeparation_distrib_L: "h \<in> (A \<heavy_asterisk> (B \<dbl_and> P)) \<Longrightarrow> h \<in> (A \<heavy_asterisk> B \<dbl_and> P)"
   using map_le_map_add map_le_trans by blast
@@ -155,9 +206,11 @@ lemma [elim!,\<nu>elim]: "Inhabited \<tort_lbrace> a \<tycolon> A \<heavy_asteri
 (* lemma [elim!,\<nu>elim]: "Inhabited (A \<dbl_and> B) \<Longrightarrow> (Inhabited A \<Longrightarrow> Inhabited B \<Longrightarrow> C) \<Longrightarrow> C"
   unfolding Inhabited_def by auto *)
 
-subsubsection \<open>Fusion and Stack Delimiter operator\<close>
+subsection \<open>Fusion and its derivatives\<close>
 
-definition Fusion :: "('a1::lrep,'b1) \<nu> \<Rightarrow> ('a2::lrep,'b2) \<nu> \<Rightarrow> ('a1 \<times> 'a2, 'b1 \<times> 'b2) \<nu>" (infixr "\<cross_product>" 70) 
+subsubsection \<open>Fusion\<close>
+
+definition Fusion :: "('a1,'b1) \<nu> \<Rightarrow> ('a2,'b2) \<nu> \<Rightarrow> ('a1 \<times> 'a2, 'b1 \<times> 'b2) \<nu>" (infixr "\<cross_product>" 70) 
   where "Fusion N M p x = (case p of (p1,p2) \<Rightarrow> case x of (x1,x2) \<Rightarrow> (p1 \<nuLinkL> N \<nuLinkR> x1) \<and> (p2 \<nuLinkL> M \<nuLinkR> x2))"
 
 lemma [simp]: "(p1,p2) \<nuLinkL> N \<cross_product> M \<nuLinkR> (x1,x2) \<longleftrightarrow> (p1 \<nuLinkL> N \<nuLinkR> x1) \<and> (p2 \<nuLinkL> M \<nuLinkR> x2)"
@@ -169,16 +222,38 @@ lemma [\<nu>intro]: "\<nu>Zero N z1 \<Longrightarrow> \<nu>Zero M z2 \<Longright
 lemma [\<nu>intro]: "\<^bold>c\<^bold>a\<^bold>s\<^bold>t x \<tycolon> N \<longmapsto> x' \<tycolon> N' \<^bold>w\<^bold>i\<^bold>t\<^bold>h P \<Longrightarrow> \<^bold>c\<^bold>a\<^bold>s\<^bold>t y \<tycolon> M \<longmapsto> y' \<tycolon> M' \<^bold>w\<^bold>i\<^bold>t\<^bold>h Q \<Longrightarrow>
   \<^bold>c\<^bold>a\<^bold>s\<^bold>t (x,y) \<tycolon> N \<cross_product> M \<longmapsto> (x',y') \<tycolon> N' \<cross_product> M' \<^bold>w\<^bold>i\<^bold>t\<^bold>h P \<and> Q" unfolding Cast_def by auto
 
+(* no_notation RepSet ("\<tort_lbrace> _ \<tort_rbrace>" [10] )
+syntax "_RepSet" :: "\<nu>typing \<Rightarrow> 'a set"  ("\<tort_lbrace> _ \<tort_rbrace>" [10] )
+translations "_RepSet A " \<rightleftharpoons> "CONST RepSet (A)"
+term "\<tort_lbrace> a \<tycolon> A\<tort_rbrace> " *)
+
+subsubsection \<open>Stack Delimiter operator\<close>
+
 definition Stack_Delimiter :: "('a::lrep,'ax) \<nu> \<Rightarrow> ('b::lrep,'bx) \<nu> \<Rightarrow> ('a \<times> 'b, 'ax \<times> 'bx) \<nu>" (infixr "<stack-div>" 70)
   where "A <stack-div> B = A \<cross_product> B"
-abbreviation Stack_Delimiter_sugar :: " ('a :: stack, 'ax) typing \<Rightarrow> ('b :: lrep, 'bx) typing \<Rightarrow> ('b \<times> 'a, 'bx \<times> 'ax) typing " ( "_/ \<heavy_comma> _" [14,15] 14)
-  where "(A \<heavy_comma> B) \<equiv> (typing_img B, typing_img A) \<tycolon> (typing_nu B <stack-div> typing_nu A)"
+consts "Stack_Delimiter_sugar" :: " 'just \<Rightarrow> 'a \<Rightarrow> 'sugar " ( "_/ \<heavy_comma> _" [14,15] 14) \<comment> \<open>Note it is left associative\<close>
+translations " a \<tycolon> A\<heavy_comma> b \<tycolon> B " == " (CONST Pair b a) \<tycolon> (B <stack-div> A) "
+  " A \<heavy_comma> B" => " (CONST Pair (_\<nu>typing_x B) (_\<nu>typing_x A)) \<tycolon> ((_\<nu>typing_ty B) <stack-div> (_\<nu>typing_ty A)) "
 
-lemma [simp]: " (a \<tycolon> A \<heavy_comma> b \<tycolon> B) = ((b,a) \<tycolon> (B <stack-div> A)) " by auto
-translations " (a \<tycolon> A) \<heavy_comma> (b \<tycolon> B) " \<rightleftharpoons> " (CONST Pair b a) \<tycolon> (B <stack-div> A) "
+lemma [simp]: "(pa,pb) \<nuLinkL> A <stack-div> B \<nuLinkR> (xa,xb) \<longleftrightarrow> (pa \<nuLinkL> A \<nuLinkR> xa) \<and> (pb \<nuLinkL> B \<nuLinkR> xb)" unfolding Stack_Delimiter_def by simp
 
 lemma [cong]: "\<tort_lbrace> a \<tycolon> A \<tort_rbrace> \<equiv> \<tort_lbrace>a' \<tycolon> A'\<tort_rbrace> \<Longrightarrow> \<tort_lbrace> b \<tycolon> B \<tort_rbrace> \<equiv> \<tort_lbrace>b' \<tycolon> B'\<tort_rbrace> \<Longrightarrow> \<tort_lbrace> a \<tycolon> A\<heavy_comma> b \<tycolon> B \<tort_rbrace> \<equiv> \<tort_lbrace> a' \<tycolon> A' \<heavy_comma> b' \<tycolon> B' \<tort_rbrace>"
   unfolding atomize_eq unfolding Stack_Delimiter_def by auto
+
+
+subsection \<open>Top Context\<close>
+
+subsubsection \<open>Context Type\<close> \<comment> \<open>The pair of heap and stack\<close>
+
+definition NuTopCtx :: " (heap, 'hx) \<nu> \<Rightarrow> ('s :: stack, 'sx) \<nu> \<Rightarrow> (heap \<times> 's, 'hx \<times> 'sx) \<nu> " (infix "<top-ctx>" 59)
+  where "(H <top-ctx> S) = (\<lambda>(hp,sp) (h,s). (hp \<nuLinkL> H \<nuLinkR> h) \<and> (sp \<nuLinkL> S \<nuLinkR> s) \<and> Heap hp)"
+consts "NuTopCtx_sugar" :: " 'just \<Rightarrow> 'a \<Rightarrow> 'sugar " ( "(2_ \<heavy_comma>/ \<^bold>h\<^bold>e\<^bold>a\<^bold>p _)" [10,14] 13)
+translations "(s \<tycolon> S\<heavy_comma> \<^bold>h\<^bold>e\<^bold>a\<^bold>p h \<tycolon> H)" \<rightleftharpoons> "(CONST Pair h s) \<tycolon> CONST NuTopCtx H S"
+  "(S\<heavy_comma> \<^bold>h\<^bold>e\<^bold>a\<^bold>p H)" => "(_\<nu>typing_x H, _\<nu>typing_x S) \<tycolon> CONST NuTopCtx (_\<nu>typing_ty H) (_\<nu>typing_ty S)"
+
+lemma [simp]: " ((hp, sp) \<nuLinkL> H <top-ctx> S  \<nuLinkR> (h, s)) \<longleftrightarrow> (hp \<nuLinkL> H  \<nuLinkR> h) \<and> (sp \<nuLinkL> S  \<nuLinkR> s) \<and> Heap hp"
+  unfolding NuTopCtx_def Refining_ex by simp
+lemma [elim!,\<nu>elim]: "Inhabited \<tort_lbrace> s \<tycolon> S \<heavy_comma> \<^bold>h\<^bold>e\<^bold>a\<^bold>p h \<tycolon> H \<tort_rbrace> \<Longrightarrow> (s \<ratio> S \<Longrightarrow> h \<ratio> H \<Longrightarrow> C) \<Longrightarrow> C" unfolding Inhabited_def by auto
 
 
 subsection \<open>Existential Nu-type\<close>
@@ -199,7 +274,7 @@ lemma [simp]: "p \<in> \<S>  \<tort_lbrace>x \<tycolon> ExNu T\<tort_rbrace> \<l
 lemma [simp]: "p \<in> \<S_S> \<tort_lbrace>x \<tycolon> ExNu T\<tort_rbrace> \<longleftrightarrow> (\<exists>z. p \<in> \<S_S> \<tort_lbrace>x z \<tycolon> T z\<tort_rbrace>)" by (auto 4 3)
 lemma [simp]: "\<tort_lbrace>x \<tycolon> ExNu T \<heavy_comma> y \<tycolon> R\<tort_rbrace> = \<tort_lbrace>\<exists>* c. x c \<tycolon> T c \<heavy_comma> y \<tycolon> R \<tort_rbrace>" unfolding Stack_Delimiter_def by auto
 lemma [simp]: "\<tort_lbrace>y \<tycolon> L \<heavy_comma> x \<tycolon> ExNu T\<tort_rbrace> = \<tort_lbrace>\<exists>* c. y \<tycolon> L \<heavy_comma> x c \<tycolon> T c \<tort_rbrace>" unfolding Stack_Delimiter_def by auto
-lemma ExTyp_strip: "(\<^bold>c\<^bold>u\<^bold>r\<^bold>r\<^bold>e\<^bold>n\<^bold>t p \<^bold>r\<^bold>e\<^bold>s\<^bold>u\<^bold>l\<^bold>t\<^bold>s \<^bold>i\<^bold>n (x \<tycolon> ExNu T)) \<equiv> (\<exists>x. \<^bold>c\<^bold>u\<^bold>r\<^bold>r\<^bold>e\<^bold>n\<^bold>t p \<^bold>r\<^bold>e\<^bold>s\<^bold>u\<^bold>l\<^bold>t\<^bold>s \<^bold>i\<^bold>n T x)"
+lemma ExTyp_strip: "(\<^bold>c\<^bold>u\<^bold>r\<^bold>r\<^bold>e\<^bold>n\<^bold>t p \<^bold>r\<^bold>e\<^bold>s\<^bold>u\<^bold>l\<^bold>t\<^bold>s \<^bold>i\<^bold>n (x \<tycolon> ExNu T)) \<equiv> (\<exists>c. \<^bold>c\<^bold>u\<^bold>r\<^bold>r\<^bold>e\<^bold>n\<^bold>t p \<^bold>r\<^bold>e\<^bold>s\<^bold>u\<^bold>l\<^bold>t\<^bold>s \<^bold>i\<^bold>n x c \<tycolon> T c)"
   unfolding CurrentConstruction_def by auto
 
 (* definition ExTyp :: "('a \<Rightarrow> 'b set) \<Rightarrow> 'b set" (binder "\<exists>* " 10)
@@ -232,24 +307,31 @@ lemma AutoExTyp_strip: "(\<^bold>c\<^bold>u\<^bold>r\<^bold>r\<^bold>e\<^bold>n\
 
 subsection \<open>Addition Nu-type : coheres true proposition\<close>
 
-definition AddtionTy :: " 'a set \<Rightarrow> bool \<Rightarrow> 'a set " (infixl "\<addition>" 50)
-  where " (T \<addition> P) = {x. x \<in> T \<and> P}"
-lemma [simp]: "T \<addition> True = T" unfolding AddtionTy_def by simp
-lemma [simp]: "x \<in> (T \<addition> P) \<longleftrightarrow> x \<in> T \<and> P" unfolding AddtionTy_def by simp
-(* lemma [intro]: "P \<Longrightarrow> [h] x \<in>\<^sub>\<nu> T \<Longrightarrow> [h] x \<in>\<^sub>\<nu> (T \<addition> P)" by simp
-lemma [elim]: "[h] x \<in>\<^sub>\<nu> (T \<addition> P) \<Longrightarrow> ([h] x \<in>\<^sub>\<nu> T \<Longrightarrow> P \<Longrightarrow> C) \<Longrightarrow> C" by simp*)
-lemma [simp]: "(R \<heavy_comma> T \<addition> P) = ((R \<heavy_comma> T) \<addition> P)" by auto
-lemma t1: "(\<^bold>c\<^bold>u\<^bold>r\<^bold>r\<^bold>e\<^bold>n\<^bold>t s \<^bold>r\<^bold>e\<^bold>s\<^bold>u\<^bold>l\<^bold>t\<^bold>s \<^bold>i\<^bold>n T \<addition> P) \<longleftrightarrow> (\<^bold>c\<^bold>u\<^bold>r\<^bold>r\<^bold>e\<^bold>n\<^bold>t s \<^bold>r\<^bold>e\<^bold>s\<^bold>u\<^bold>l\<^bold>t\<^bold>s \<^bold>i\<^bold>n T) \<and> P" unfolding CurrentConstruction_def by (cases s) auto
-lemma [simp]: "((((\<^bold>c\<^bold>u\<^bold>r\<^bold>r\<^bold>e\<^bold>n\<^bold>t s \<^bold>r\<^bold>e\<^bold>s\<^bold>u\<^bold>l\<^bold>t\<^bold>s \<^bold>i\<^bold>n S) \<and> B) \<and> C) \<^bold>w\<^bold>i\<^bold>t\<^bold>h \<^bold>f\<^bold>a\<^bold>c\<^bold>t\<^bold>s: PROP L) \<equiv> (((\<^bold>c\<^bold>u\<^bold>r\<^bold>r\<^bold>e\<^bold>n\<^bold>t s \<^bold>r\<^bold>e\<^bold>s\<^bold>u\<^bold>l\<^bold>t\<^bold>s \<^bold>i\<^bold>n S) \<and> (B \<and> C)) \<^bold>w\<^bold>i\<^bold>t\<^bold>h \<^bold>f\<^bold>a\<^bold>c\<^bold>t\<^bold>s: PROP L)" by simp
+definition NuAddition :: " ('p,'x) \<nu> \<Rightarrow> bool \<Rightarrow> ('p,'x) \<nu> " (infixl "\<and>\<^sup>\<nu>" 50)
+  where " (N \<and>\<^sup>\<nu> P) = (\<lambda>p x. P \<and> (p \<nuLinkL> N \<nuLinkR> x))"
+translations "(x \<tycolon> T) \<and> P" \<rightleftharpoons> "x \<tycolon> T \<and>\<^sup>\<nu> P"
+lemma [simp]: "p \<nuLinkL> T \<and>\<^sup>\<nu> P \<nuLinkR> x \<longleftrightarrow> P \<and> (p \<nuLinkL> T \<nuLinkR> x)" unfolding NuAddition_def Refining_ex ..
+
+lemma [simp]: "\<tort_lbrace> x \<tycolon> T \<and>\<^sup>\<nu> True\<tort_rbrace> = \<tort_lbrace> x \<tycolon> T \<tort_rbrace>" by auto
+lemma [simp]: "\<tort_lbrace>L \<heavy_comma> (x \<tycolon> T) \<and> P\<tort_rbrace> = \<tort_lbrace>(L \<heavy_comma> x \<tycolon> T) \<and> P\<tort_rbrace>" and [simp]: "\<tort_lbrace>(x \<tycolon> T) \<and> P\<heavy_comma> R\<tort_rbrace> = \<tort_lbrace>(x \<tycolon> T\<heavy_comma> R) \<and> P\<tort_rbrace>"
+  unfolding Stack_Delimiter_def by auto
+lemma [simp]: "\<tort_lbrace>L \<heavy_asterisk> (x \<tycolon> T) \<and> P\<tort_rbrace> = \<tort_lbrace>(L \<heavy_asterisk> x \<tycolon> T) \<and> P\<tort_rbrace>" and [simp]: "\<tort_lbrace>(x \<tycolon> T) \<and> P\<heavy_asterisk> R\<tort_rbrace> = \<tort_lbrace>(x \<tycolon> T\<heavy_asterisk> R) \<and> P\<tort_rbrace>"
+  unfolding Heap_Delimiter_def by auto blast+
+lemma [simp]: "\<tort_lbrace> (s \<tycolon> S) \<and> P \<heavy_comma> \<^bold>h\<^bold>e\<^bold>a\<^bold>p h \<tycolon> H \<tort_rbrace> = \<tort_lbrace> (s \<tycolon> S\<heavy_comma> \<^bold>h\<^bold>e\<^bold>a\<^bold>p h \<tycolon> H) \<and> P \<tort_rbrace>"
+  and [simp]: "\<tort_lbrace> s \<tycolon> S \<heavy_comma> \<^bold>h\<^bold>e\<^bold>a\<^bold>p (h \<tycolon> H) \<and> P \<tort_rbrace> = \<tort_lbrace> (s \<tycolon> S\<heavy_comma> \<^bold>h\<^bold>e\<^bold>a\<^bold>p h \<tycolon> H) \<and> P \<tort_rbrace>" by auto
+
+
+lemma t1: "(\<^bold>c\<^bold>u\<^bold>r\<^bold>r\<^bold>e\<^bold>n\<^bold>t s \<^bold>r\<^bold>e\<^bold>s\<^bold>u\<^bold>l\<^bold>t\<^bold>s \<^bold>i\<^bold>n (x \<tycolon> T) \<and> P) \<longleftrightarrow> (\<^bold>c\<^bold>u\<^bold>r\<^bold>r\<^bold>e\<^bold>n\<^bold>t s \<^bold>r\<^bold>e\<^bold>s\<^bold>u\<^bold>l\<^bold>t\<^bold>s \<^bold>i\<^bold>n x \<tycolon> T) \<and> P" unfolding CurrentConstruction_def by (cases s) auto
+lemma [simp]: "((((\<^bold>c\<^bold>u\<^bold>r\<^bold>r\<^bold>e\<^bold>n\<^bold>t s \<^bold>r\<^bold>e\<^bold>s\<^bold>u\<^bold>l\<^bold>t\<^bold>s \<^bold>i\<^bold>n T) \<and> B) \<and> C) \<^bold>w\<^bold>i\<^bold>t\<^bold>h \<^bold>f\<^bold>a\<^bold>c\<^bold>t\<^bold>s: PROP L) \<equiv> (((\<^bold>c\<^bold>u\<^bold>r\<^bold>r\<^bold>e\<^bold>n\<^bold>t s \<^bold>r\<^bold>e\<^bold>s\<^bold>u\<^bold>l\<^bold>t\<^bold>s \<^bold>i\<^bold>n T) \<and> (B \<and> C)) \<^bold>w\<^bold>i\<^bold>t\<^bold>h \<^bold>f\<^bold>a\<^bold>c\<^bold>t\<^bold>s: PROP L)" by simp
 
 lemma move_fact_to_star1[simp]:
-  "((\<^bold>c\<^bold>u\<^bold>r\<^bold>r\<^bold>e\<^bold>n\<^bold>t s \<^bold>r\<^bold>e\<^bold>s\<^bold>u\<^bold>l\<^bold>t\<^bold>s \<^bold>i\<^bold>n S \<addition> Q) \<^bold>w\<^bold>i\<^bold>t\<^bold>h \<^bold>f\<^bold>a\<^bold>c\<^bold>t\<^bold>s: PROP FactCollection (PROP NoFact) (PROP L) (PROP I))
-    \<Longrightarrow> (\<^bold>c\<^bold>u\<^bold>r\<^bold>r\<^bold>e\<^bold>n\<^bold>t s \<^bold>r\<^bold>e\<^bold>s\<^bold>u\<^bold>l\<^bold>t\<^bold>s \<^bold>i\<^bold>n S \<^bold>w\<^bold>i\<^bold>t\<^bold>h \<^bold>f\<^bold>a\<^bold>c\<^bold>t\<^bold>s: PROP FactCollection (Trueprop Q) (PROP L) (PROP I))"
+  "((\<^bold>c\<^bold>u\<^bold>r\<^bold>r\<^bold>e\<^bold>n\<^bold>t s \<^bold>r\<^bold>e\<^bold>s\<^bold>u\<^bold>l\<^bold>t\<^bold>s \<^bold>i\<^bold>n (x \<tycolon> T) \<and> Q) \<^bold>w\<^bold>i\<^bold>t\<^bold>h \<^bold>f\<^bold>a\<^bold>c\<^bold>t\<^bold>s: PROP FactCollection (PROP NoFact) (PROP L) (PROP I))
+    \<Longrightarrow> (\<^bold>c\<^bold>u\<^bold>r\<^bold>r\<^bold>e\<^bold>n\<^bold>t s \<^bold>r\<^bold>e\<^bold>s\<^bold>u\<^bold>l\<^bold>t\<^bold>s \<^bold>i\<^bold>n x \<tycolon> T \<^bold>w\<^bold>i\<^bold>t\<^bold>h \<^bold>f\<^bold>a\<^bold>c\<^bold>t\<^bold>s: PROP FactCollection (Trueprop Q) (PROP L) (PROP I))"
   unfolding t1 SpecTop_imp conj_imp FactCollection_imp
   by (intro equal_intr_rule SpecTop_I FactCollection_I conjI NoFact) (* (unfold SpecTop_imp conj_imp FactCollection_imp) *)
 lemma move_fact_to_star2[simp]:
-  "((\<^bold>c\<^bold>u\<^bold>r\<^bold>r\<^bold>e\<^bold>n\<^bold>t s \<^bold>r\<^bold>e\<^bold>s\<^bold>u\<^bold>l\<^bold>t\<^bold>s \<^bold>i\<^bold>n S \<addition> Q) \<^bold>w\<^bold>i\<^bold>t\<^bold>h \<^bold>f\<^bold>a\<^bold>c\<^bold>t\<^bold>s: PROP FactCollection (Trueprop P) (PROP L) (PROP I))
-    \<Longrightarrow> (\<^bold>c\<^bold>u\<^bold>r\<^bold>r\<^bold>e\<^bold>n\<^bold>t s \<^bold>r\<^bold>e\<^bold>s\<^bold>u\<^bold>l\<^bold>t\<^bold>s \<^bold>i\<^bold>n S \<^bold>w\<^bold>i\<^bold>t\<^bold>h \<^bold>f\<^bold>a\<^bold>c\<^bold>t\<^bold>s: PROP FactCollection  (Trueprop (Q \<and> P)) (PROP L) (PROP I))"
+  "((\<^bold>c\<^bold>u\<^bold>r\<^bold>r\<^bold>e\<^bold>n\<^bold>t s \<^bold>r\<^bold>e\<^bold>s\<^bold>u\<^bold>l\<^bold>t\<^bold>s \<^bold>i\<^bold>n (x \<tycolon> T) \<and> Q) \<^bold>w\<^bold>i\<^bold>t\<^bold>h \<^bold>f\<^bold>a\<^bold>c\<^bold>t\<^bold>s: PROP FactCollection (Trueprop P) (PROP L) (PROP I))
+    \<Longrightarrow> (\<^bold>c\<^bold>u\<^bold>r\<^bold>r\<^bold>e\<^bold>n\<^bold>t s \<^bold>r\<^bold>e\<^bold>s\<^bold>u\<^bold>l\<^bold>t\<^bold>s \<^bold>i\<^bold>n x \<tycolon> T \<^bold>w\<^bold>i\<^bold>t\<^bold>h \<^bold>f\<^bold>a\<^bold>c\<^bold>t\<^bold>s: PROP FactCollection  (Trueprop (Q \<and> P)) (PROP L) (PROP I))"
   unfolding t1 SpecTop_imp conj_imp FactCollection_imp
   by (intro equal_intr_rule SpecTop_I FactCollection_I conjI) (* (unfold SpecTop_imp conj_imp FactCollection_imp) *)
 
@@ -275,52 +357,19 @@ next fix x assume "\<And>a b. PROP P (a \<R_arr_tail> b)"
     from \<open>PROP P (key_of x \<R_arr_tail> val_of x)\<close> show "PROP P x" by simp
 qed
 
-subsection \<open>Argument and return list\<close>
-
-consts "Arg_Ret_Pair_sugar" :: " (heap \<times> 'a::lrep) set \<Rightarrow> (heap \<times> 'b::lrep) set \<Rightarrow> 'wow_sugar" (infix "\<longmapsto>" 2)
-
-ML \<open>local open Ast in
-  fun tr_pair_i ret (Appl [Constant \<^syntax_const>\<open>_tuple_args\<close>, X, Y])
-        = tr_pair_i (Appl [Constant \<^const_syntax>\<open>Stack_Delimiter\<close>, ret, X]) Y
-    | tr_pair_i ret (Appl [Constant \<^syntax_const>\<open>_tuple_arg\<close>, y])
-        = Appl [Constant \<^const_syntax>\<open>Stack_Delimiter\<close>, ret, y]
-  fun tr_pair (Appl [Constant \<^syntax_const>\<open>_tuple\<close>, X, Y]) = tr_pair_i X Y
-    | tr_pair x = x
-  fun tr_stack (Appl [Constant \<^const_syntax>\<open>Stack_Delimiter\<close>, X, Y])
-        = Appl [Constant \<^const_syntax>\<open>Stack_Delimiter\<close>, tr_stack X, Y]
-    | tr_stack (a as Appl [Constant \<^const_syntax>\<open>typing\<close>, _, _])
-        = Appl [Constant \<^const_syntax>\<open>Stack_Delimiter\<close>, Variable "\<R>", a]
-    | tr_stack variable = variable
-  val tr_stack_final = tr_stack o tr_pair
-  fun tr_context (Appl [Constant \<^const_syntax>\<open>Context\<close>, X, Y])
-        = (Appl [Constant \<^const_syntax>\<open>Context\<close>, tr_stack_final X, Y])
-    | tr_context (X as Appl [Constant \<^const_syntax>\<open>Stack_Delimiter\<close>, _, _])
-        = (Appl [Constant \<^const_syntax>\<open>Context\<close>, tr_stack_final X, Variable "\<H>"])
-    | tr_context (X as Appl [Constant \<^const_syntax>\<open>typing\<close>, _, _])
-        = (Appl [Constant \<^const_syntax>\<open>Context\<close>, tr_stack_final X, Variable "\<H>"])
-    | tr_context v = v
-  fun tr_context_final x = tr_context (tr_pair x)
-  fun tr_proc ([f, T, U])
-    = (Appl [Constant \<^const_syntax>\<open>Procedure\<close>, f, tr_context_final T, tr_context_final U])
-  fun tr_arg_ret_pair ([T, U])
-    = (Appl [Constant \<^const_syntax>\<open>Arg_Ret_Pair_sugar\<close>, tr_context_final T, tr_context_final U])
-end\<close>
-
-parse_ast_translation \<open>[
-  (\<^const_syntax>\<open>Procedure\<close>, K tr_proc),
-  (\<^const_syntax>\<open>Arg_Ret_Pair_sugar\<close>, K tr_arg_ret_pair)
-]\<close>
 
 section \<open>Mechanisms - II\<close>
 
 
-
 subsection \<open>Heap\<close>
 
-definition Nothing :: "heap set" where  "Nothing = {Map.empty}"
-term "Map.empty"
-lemma Separation_emptyL: "(Nothing \<heavy_asterisk> S) = S" and Separation_emptyR: "(S \<heavy_asterisk> Nothing) = S"
-  unfolding Nothing_def Separation_def by auto
+definition NuNothing :: "(heap, unit) \<nu>" where  "NuNothing h x \<longleftrightarrow> h = Map.empty"
+consts Nothing_sugar :: " 'a_sugar " ("Nothing")
+translations "Nothing" \<rightleftharpoons> "() \<tycolon> CONST NuNothing"
+lemma [simp]: "h \<nuLinkL> NuNothing \<nuLinkR> x \<longleftrightarrow> h = Map.empty" unfolding Refining_ex NuNothing_def by simp
+
+lemma Separation_emptyL: "\<tort_lbrace>Nothing \<heavy_asterisk> h \<tycolon> H\<tort_rbrace> = \<tort_lbrace>h \<tycolon> H\<tort_rbrace>" and Separation_emptyR: "\<tort_lbrace>h \<tycolon> H \<heavy_asterisk> Nothing\<tort_rbrace> = \<tort_lbrace>h \<tycolon> H\<tort_rbrace>"
+  unfolding Heap_Delimiter_def by auto
 
 subsubsection \<open>Syntax & Auxiliary\<close>
 
@@ -371,10 +420,9 @@ lemma MemAddrState_retained_S[intro]:
 *)
 
 
-lemma MemAddrState_restrict_I1[intro]: "h \<^bold>a\<^bold>t a \<^bold>i\<^bold>s T \<Longrightarrow> a \<in> S \<Longrightarrow> h |` (MemAddress ` S) \<^bold>a\<^bold>t a \<^bold>i\<^bold>s T "
-  and MemAddrState_restrict_I2[intro]: "h \<^bold>a\<^bold>t a \<^bold>i\<^bold>s T \<Longrightarrow> a \<notin> S \<Longrightarrow> h |` (- MemAddress ` S) \<^bold>a\<^bold>t a \<^bold>i\<^bold>s T "
-  unfolding MemAddrState_def addr_allocated_def
-  by auto (metis ComplI imageE option.sel resource_key.inject(1) restrict_map_def)
+lemma MemAddrState_restrict_I1[intro]: "h \<^bold>a\<^bold>t a \<^bold>i\<^bold>s T \<Longrightarrow> MemAddress a \<in> S \<Longrightarrow> h |` S \<^bold>a\<^bold>t a \<^bold>i\<^bold>s T "
+  and MemAddrState_restrict_I2[intro]: "h \<^bold>a\<^bold>t a \<^bold>i\<^bold>s T \<Longrightarrow> MemAddress a \<notin> S \<Longrightarrow> h |` (- S) \<^bold>a\<^bold>t a \<^bold>i\<^bold>s T "
+  unfolding MemAddrState_def addr_allocated_def by auto
 
 lemma MemAddrState_add_I1[intro]: " h1 \<^bold>a\<^bold>t a \<^bold>i\<^bold>s T \<Longrightarrow> dom h1 \<perpendicular> dom h2 \<Longrightarrow> h1 ++ h2 \<^bold>a\<^bold>t a \<^bold>i\<^bold>s T "
   and  MemAddrState_add_I2[intro]: " h2 \<^bold>a\<^bold>t a \<^bold>i\<^bold>s T \<Longrightarrow> dom h1 \<perpendicular> dom h2 \<Longrightarrow> h1 ++ h2 \<^bold>a\<^bold>t a \<^bold>i\<^bold>s T "
@@ -383,20 +431,19 @@ lemma MemAddrState_add_I1[intro]: " h1 \<^bold>a\<^bold>t a \<^bold>i\<^bold>s T
 
 subsubsection \<open>Cast\<close>
 
-definition Heap_Cast_Goal :: " heap set \<Rightarrow> heap set " ("\<medium_left_bracket> _ \<medium_right_bracket>") where "Heap_Cast_Goal x = x"
+definition Heap_Cast_Goal :: " (heap, 'x) \<nu> \<Rightarrow> (heap, 'x) \<nu> "  ("\<medium_left_bracket> _ \<medium_right_bracket>") where "Heap_Cast_Goal x = x"
   \<comment> \<open>The protector marks the goal to be gained\<close>
-translations "\<medium_left_bracket> x \<tycolon> T \<medium_right_bracket>" \<rightleftharpoons> "\<medium_left_bracket> \<tort_lbrace> x \<tycolon> T \<tort_rbrace> \<medium_right_bracket>"
 
-lemma [\<nu>intro0]: "\<^bold>c\<^bold>a\<^bold>s\<^bold>t H \<longmapsto> \<medium_left_bracket> H \<medium_right_bracket> \<^bold>d\<^bold>u\<^bold>a\<^bold>l \<medium_left_bracket> H\<^sub>m \<medium_right_bracket> \<longmapsto> H\<^sub>m" unfolding Heap_Cast_Goal_def using cast_dual_id .
+lemma [\<nu>intro0]: "\<^bold>c\<^bold>a\<^bold>s\<^bold>t h \<tycolon> H \<longmapsto> h \<tycolon> \<medium_left_bracket> H \<medium_right_bracket> \<^bold>d\<^bold>u\<^bold>a\<^bold>l h\<^sub>m \<tycolon> \<medium_left_bracket> H\<^sub>m \<medium_right_bracket> \<longmapsto> h\<^sub>m \<tycolon> H\<^sub>m" unfolding Heap_Cast_Goal_def using cast_dual_id .
 
 lemma context_cast[\<nu>intro]:
-  "\<^bold>c\<^bold>a\<^bold>s\<^bold>t K \<longmapsto> K' \<^bold>w\<^bold>i\<^bold>t\<^bold>h P \<Longrightarrow> \<^bold>c\<^bold>a\<^bold>s\<^bold>t H \<longmapsto> \<medium_left_bracket> H' \<medium_right_bracket> \<^bold>w\<^bold>i\<^bold>t\<^bold>h Q \<Longrightarrow> \<^bold>c\<^bold>a\<^bold>s\<^bold>t (K\<heavy_comma> \<^bold>h\<^bold>e\<^bold>a\<^bold>p H) \<longmapsto> (K'\<heavy_comma> \<^bold>h\<^bold>e\<^bold>a\<^bold>p H') \<^bold>w\<^bold>i\<^bold>t\<^bold>h P \<and> Q"
+  "\<^bold>c\<^bold>a\<^bold>s\<^bold>t k \<tycolon> K \<longmapsto> k' \<tycolon> K' \<^bold>w\<^bold>i\<^bold>t\<^bold>h P \<Longrightarrow> \<^bold>c\<^bold>a\<^bold>s\<^bold>t h \<tycolon> H \<longmapsto> h' \<tycolon> \<medium_left_bracket> H' \<medium_right_bracket> \<^bold>w\<^bold>i\<^bold>t\<^bold>h Q \<Longrightarrow> \<^bold>c\<^bold>a\<^bold>s\<^bold>t (k \<tycolon> K\<heavy_comma> \<^bold>h\<^bold>e\<^bold>a\<^bold>p h \<tycolon> H) \<longmapsto> (k' \<tycolon> K'\<heavy_comma> \<^bold>h\<^bold>e\<^bold>a\<^bold>p h' \<tycolon> H') \<^bold>w\<^bold>i\<^bold>t\<^bold>h P \<and> Q"
   unfolding Cast_def Heap_Cast_Goal_def by (auto simp add: pair_forall)
 
 lemma context_cast_dual[\<nu>intro]:
-  "\<^bold>c\<^bold>a\<^bold>s\<^bold>t K \<longmapsto> K' \<^bold>w\<^bold>i\<^bold>t\<^bold>h PK
-    \<Longrightarrow> \<^bold>c\<^bold>a\<^bold>s\<^bold>t H \<longmapsto> \<medium_left_bracket> H' \<medium_right_bracket> \<^bold>w\<^bold>i\<^bold>t\<^bold>h PH \<^bold>d\<^bold>u\<^bold>a\<^bold>l \<medium_left_bracket> H2 \<medium_right_bracket> \<longmapsto> H2' \<^bold>w\<^bold>h\<^bold>e\<^bold>n QH
-    \<Longrightarrow> \<^bold>c\<^bold>a\<^bold>s\<^bold>t (K\<heavy_comma> \<^bold>h\<^bold>e\<^bold>a\<^bold>p H) \<longmapsto> (K'\<heavy_comma> \<^bold>h\<^bold>e\<^bold>a\<^bold>p H') \<^bold>w\<^bold>i\<^bold>t\<^bold>h PK \<and> PH \<^bold>d\<^bold>u\<^bold>a\<^bold>l (K2\<heavy_comma> \<^bold>h\<^bold>e\<^bold>a\<^bold>p H2) \<longmapsto> (K2\<heavy_comma> \<^bold>h\<^bold>e\<^bold>a\<^bold>p H2') \<^bold>w\<^bold>h\<^bold>e\<^bold>n QH"
+  "\<^bold>c\<^bold>a\<^bold>s\<^bold>t k \<tycolon> K \<longmapsto> k' \<tycolon> K' \<^bold>w\<^bold>i\<^bold>t\<^bold>h PK
+    \<Longrightarrow> \<^bold>c\<^bold>a\<^bold>s\<^bold>t h \<tycolon> H \<longmapsto> h' \<tycolon> \<medium_left_bracket> H' \<medium_right_bracket> \<^bold>w\<^bold>i\<^bold>t\<^bold>h PH \<^bold>d\<^bold>u\<^bold>a\<^bold>l h2 \<tycolon> \<medium_left_bracket> H2 \<medium_right_bracket> \<longmapsto> h2' \<tycolon> H2' \<^bold>w\<^bold>h\<^bold>e\<^bold>n QH
+    \<Longrightarrow> \<^bold>c\<^bold>a\<^bold>s\<^bold>t (k \<tycolon> K\<heavy_comma> \<^bold>h\<^bold>e\<^bold>a\<^bold>p h \<tycolon> H) \<longmapsto> (k' \<tycolon> K'\<heavy_comma> \<^bold>h\<^bold>e\<^bold>a\<^bold>p h' \<tycolon> H') \<^bold>w\<^bold>i\<^bold>t\<^bold>h PK \<and> PH \<^bold>d\<^bold>u\<^bold>a\<^bold>l (k2 \<tycolon> K2\<heavy_comma> \<^bold>h\<^bold>e\<^bold>a\<^bold>p h2 \<tycolon> H2) \<longmapsto> (k2 \<tycolon> K2\<heavy_comma> \<^bold>h\<^bold>e\<^bold>a\<^bold>p h2' \<tycolon> H2') \<^bold>w\<^bold>h\<^bold>e\<^bold>n QH"
   unfolding CastDual_def Cast_def Heap_Cast_Goal_def by (auto simp add: pair_forall)
 
 (* lemma [\<nu>intro0]: "\<^bold>c\<^bold>a\<^bold>s\<^bold>t x \<tycolon> X \<longmapsto> H' \<heavy_asterisk> y \<tycolon> Y \<^bold>w\<^bold>i\<^bold>t\<^bold>h P \<^bold>d\<^bold>u\<^bold>a\<^bold>l H'\<^sub>m \<heavy_asterisk> y\<^sub>m \<tycolon> Y \<longmapsto> x\<^sub>m \<tycolon> X \<^bold>w\<^bold>h\<^bold>e\<^bold>n Q
@@ -404,53 +451,55 @@ lemma context_cast_dual[\<nu>intro]:
   unfolding Heap_Cast_Goal_def . *)
 (* lemma [\<nu>intro0]: "\<^bold>c\<^bold>a\<^bold>s\<^bold>t A \<longmapsto> A \<^bold>d\<^bold>u\<^bold>a\<^bold>l B \<longmapsto> B" unfolding CastDual_def  by (simp add: cast_id) *)
 
-lemma [\<nu>intro0]: "\<^bold>c\<^bold>a\<^bold>s\<^bold>t L \<heavy_asterisk> H \<longmapsto> L \<heavy_asterisk> \<medium_left_bracket> H \<medium_right_bracket> \<^bold>d\<^bold>u\<^bold>a\<^bold>l L \<heavy_asterisk> \<medium_left_bracket> H\<^sub>m \<medium_right_bracket> \<longmapsto> L \<heavy_asterisk> H\<^sub>m" unfolding Heap_Cast_Goal_def using cast_dual_id .
+lemma [\<nu>intro0]: "\<^bold>c\<^bold>a\<^bold>s\<^bold>t L \<heavy_asterisk> h \<tycolon> H \<longmapsto> L \<heavy_asterisk> h \<tycolon> \<medium_left_bracket> H \<medium_right_bracket> \<^bold>d\<^bold>u\<^bold>a\<^bold>l L \<heavy_asterisk> h\<^sub>m \<tycolon> \<medium_left_bracket> H\<^sub>m \<medium_right_bracket> \<longmapsto> L \<heavy_asterisk> h\<^sub>m \<tycolon> H\<^sub>m" unfolding Heap_Cast_Goal_def using cast_dual_id .
 
 lemma heap_idx_this[\<nu>intro]:
-  "\<^bold>c\<^bold>a\<^bold>s\<^bold>t X \<longmapsto> Nothing \<heavy_asterisk> \<medium_left_bracket> X \<medium_right_bracket> \<^bold>d\<^bold>u\<^bold>a\<^bold>l Nothing \<heavy_asterisk> \<medium_left_bracket> X\<^sub>m \<medium_right_bracket> \<longmapsto> X\<^sub>m"
+  "\<^bold>c\<^bold>a\<^bold>s\<^bold>t x \<tycolon> X \<longmapsto> Nothing \<heavy_asterisk> x \<tycolon> \<medium_left_bracket> X \<medium_right_bracket> \<^bold>d\<^bold>u\<^bold>a\<^bold>l Nothing \<heavy_asterisk> x\<^sub>m \<tycolon> \<medium_left_bracket> X\<^sub>m \<medium_right_bracket> \<longmapsto> x\<^sub>m \<tycolon> X\<^sub>m"
   unfolding Cast_def Separation_emptyL Heap_Cast_Goal_def CastDual_def by simp
 
 lemma heap_idx_L[\<nu>intro0]:
-  "\<^bold>c\<^bold>a\<^bold>s\<^bold>t S \<longmapsto> S' \<heavy_asterisk> \<medium_left_bracket> X \<medium_right_bracket> \<^bold>w\<^bold>i\<^bold>t\<^bold>h P \<^bold>d\<^bold>u\<^bold>a\<^bold>l S'\<^sub>m \<heavy_asterisk> \<medium_left_bracket> X\<^sub>m \<medium_right_bracket> \<longmapsto> S\<^sub>m \<^bold>w\<^bold>h\<^bold>e\<^bold>n Q
-    \<Longrightarrow> \<^bold>c\<^bold>a\<^bold>s\<^bold>t L \<heavy_asterisk> S \<longmapsto> L \<heavy_asterisk> S' \<heavy_asterisk> \<medium_left_bracket> X \<medium_right_bracket> \<^bold>w\<^bold>i\<^bold>t\<^bold>h P \<^bold>d\<^bold>u\<^bold>a\<^bold>l L \<heavy_asterisk> S'\<^sub>m \<heavy_asterisk> \<medium_left_bracket> X\<^sub>m \<medium_right_bracket> \<longmapsto> L \<heavy_asterisk> S\<^sub>m \<^bold>w\<^bold>h\<^bold>e\<^bold>n Q"
-  unfolding Cast_def CastDual_def Heap_Cast_Goal_def
-  by (smt (verit, del_insts) Separation_assoc Separation_comm Separation_def mem_Collect_eq)
+  "\<^bold>c\<^bold>a\<^bold>s\<^bold>t h \<tycolon> H \<longmapsto> h' \<tycolon> H' \<heavy_asterisk> x \<tycolon> \<medium_left_bracket> X \<medium_right_bracket> \<^bold>w\<^bold>i\<^bold>t\<^bold>h P \<^bold>d\<^bold>u\<^bold>a\<^bold>l h'\<^sub>m \<tycolon> H'\<^sub>m \<heavy_asterisk> x\<^sub>m \<tycolon> \<medium_left_bracket> X\<^sub>m \<medium_right_bracket> \<longmapsto> h\<^sub>m \<tycolon> H\<^sub>m \<^bold>w\<^bold>h\<^bold>e\<^bold>n Q
+    \<Longrightarrow> \<^bold>c\<^bold>a\<^bold>s\<^bold>t l \<tycolon> L \<heavy_asterisk> h \<tycolon> H \<longmapsto> l \<tycolon> L \<heavy_asterisk> h' \<tycolon> H' \<heavy_asterisk> x \<tycolon> \<medium_left_bracket> X \<medium_right_bracket> \<^bold>w\<^bold>i\<^bold>t\<^bold>h P \<^bold>d\<^bold>u\<^bold>a\<^bold>l l \<tycolon> L \<heavy_asterisk> h'\<^sub>m \<tycolon> H'\<^sub>m \<heavy_asterisk> x\<^sub>m \<tycolon> \<medium_left_bracket> X\<^sub>m \<medium_right_bracket> \<longmapsto> l \<tycolon> L \<heavy_asterisk> h\<^sub>m \<tycolon> H\<^sub>m \<^bold>w\<^bold>h\<^bold>e\<^bold>n Q"
+  unfolding Cast_def CastDual_def Heap_Cast_Goal_def SepNu_2_SepSet
+  by (smt (verit, del_insts) SeparationSet_assoc SeparationSet_comm SeparationSet_def mem_Collect_eq)
 
 lemma heap_idx_R[\<nu>intro]:
-  "\<^bold>c\<^bold>a\<^bold>s\<^bold>t S \<longmapsto> S' \<heavy_asterisk> \<medium_left_bracket> X \<medium_right_bracket> \<^bold>w\<^bold>i\<^bold>t\<^bold>h P \<^bold>d\<^bold>u\<^bold>a\<^bold>l S'\<^sub>m \<heavy_asterisk> \<medium_left_bracket> X\<^sub>m \<medium_right_bracket> \<longmapsto> S\<^sub>m \<^bold>w\<^bold>h\<^bold>e\<^bold>n Q
-    \<Longrightarrow> \<^bold>c\<^bold>a\<^bold>s\<^bold>t S \<heavy_asterisk> R \<longmapsto> S' \<heavy_asterisk> R \<heavy_asterisk> \<medium_left_bracket> X \<medium_right_bracket> \<^bold>w\<^bold>i\<^bold>t\<^bold>h P \<^bold>d\<^bold>u\<^bold>a\<^bold>l S'\<^sub>m \<heavy_asterisk> R \<heavy_asterisk> \<medium_left_bracket> X\<^sub>m \<medium_right_bracket> \<longmapsto> S\<^sub>m \<heavy_asterisk> \<medium_left_bracket> R \<medium_right_bracket> \<^bold>w\<^bold>h\<^bold>e\<^bold>n Q"
-  unfolding Cast_def CastDual_def Heap_Cast_Goal_def
-  by (smt (verit, del_insts) Separation_assoc Separation_comm Separation_def mem_Collect_eq)
+  "\<^bold>c\<^bold>a\<^bold>s\<^bold>t h \<tycolon> H \<longmapsto> h' \<tycolon> H' \<heavy_asterisk> x \<tycolon> \<medium_left_bracket> X \<medium_right_bracket> \<^bold>w\<^bold>i\<^bold>t\<^bold>h P \<^bold>d\<^bold>u\<^bold>a\<^bold>l h'\<^sub>m \<tycolon> H'\<^sub>m \<heavy_asterisk> x\<^sub>m \<tycolon> \<medium_left_bracket> X\<^sub>m \<medium_right_bracket> \<longmapsto> h\<^sub>m \<tycolon> H\<^sub>m \<^bold>w\<^bold>h\<^bold>e\<^bold>n Q
+    \<Longrightarrow> \<^bold>c\<^bold>a\<^bold>s\<^bold>t h \<tycolon> H \<heavy_asterisk> r \<tycolon> R \<longmapsto> h' \<tycolon> H' \<heavy_asterisk> r \<tycolon> R \<heavy_asterisk> x \<tycolon> \<medium_left_bracket> X \<medium_right_bracket> \<^bold>w\<^bold>i\<^bold>t\<^bold>h P \<^bold>d\<^bold>u\<^bold>a\<^bold>l h'\<^sub>m \<tycolon> H'\<^sub>m \<heavy_asterisk> r \<tycolon> R \<heavy_asterisk> x\<^sub>m \<tycolon> \<medium_left_bracket> X\<^sub>m \<medium_right_bracket> \<longmapsto> h\<^sub>m \<tycolon> H\<^sub>m \<heavy_asterisk> r \<tycolon> \<medium_left_bracket> R \<medium_right_bracket> \<^bold>w\<^bold>h\<^bold>e\<^bold>n Q"
+  unfolding Cast_def CastDual_def Heap_Cast_Goal_def SepNu_2_SepSet
+  by (smt (verit, del_insts) SeparationSet_assoc SeparationSet_comm SeparationSet_def mem_Collect_eq)
 
 lemma [\<nu>intro]:
-  "\<^bold>c\<^bold>a\<^bold>s\<^bold>t S \<longmapsto> S1 \<heavy_asterisk> \<medium_left_bracket> X \<medium_right_bracket> \<^bold>w\<^bold>i\<^bold>t\<^bold>h P1 \<^bold>d\<^bold>u\<^bold>a\<^bold>l S1\<^sub>m \<heavy_asterisk> \<medium_left_bracket> X\<^sub>m \<medium_right_bracket> \<longmapsto> S\<^sub>m \<^bold>w\<^bold>h\<^bold>e\<^bold>n Q1
-    \<Longrightarrow> \<^bold>c\<^bold>a\<^bold>s\<^bold>t S1 \<longmapsto> \<medium_left_bracket> S2 \<medium_right_bracket> \<^bold>w\<^bold>i\<^bold>t\<^bold>h P2 \<^bold>d\<^bold>u\<^bold>a\<^bold>l \<medium_left_bracket> S2\<^sub>m \<medium_right_bracket> \<longmapsto> S1\<^sub>m \<^bold>w\<^bold>h\<^bold>e\<^bold>n Q2
-    \<Longrightarrow> \<^bold>c\<^bold>a\<^bold>s\<^bold>t S \<longmapsto> \<medium_left_bracket> S2 \<heavy_asterisk> X \<medium_right_bracket> \<^bold>w\<^bold>i\<^bold>t\<^bold>h P1 \<and> P2 \<^bold>d\<^bold>u\<^bold>a\<^bold>l \<medium_left_bracket> S2\<^sub>m \<heavy_asterisk> X\<^sub>m \<medium_right_bracket> \<longmapsto> S\<^sub>m \<^bold>w\<^bold>h\<^bold>e\<^bold>n Q1 \<and> Q2"
-  unfolding Cast_def CastDual_def Heap_Cast_Goal_def
-  by (smt (verit, del_insts) Separation_assoc Separation_comm Separation_def mem_Collect_eq)
+  "\<^bold>c\<^bold>a\<^bold>s\<^bold>t h \<tycolon> H \<longmapsto> h1 \<tycolon> H1 \<heavy_asterisk> x \<tycolon> \<medium_left_bracket> X \<medium_right_bracket> \<^bold>w\<^bold>i\<^bold>t\<^bold>h P1 \<^bold>d\<^bold>u\<^bold>a\<^bold>l h1\<^sub>m \<tycolon> H1\<^sub>m \<heavy_asterisk> x\<^sub>m \<tycolon> \<medium_left_bracket> X\<^sub>m \<medium_right_bracket> \<longmapsto> h\<^sub>m \<tycolon> H\<^sub>m \<^bold>w\<^bold>h\<^bold>e\<^bold>n Q1
+    \<Longrightarrow> \<^bold>c\<^bold>a\<^bold>s\<^bold>t h1 \<tycolon> H1 \<longmapsto> h2 \<tycolon> \<medium_left_bracket> H2 \<medium_right_bracket> \<^bold>w\<^bold>i\<^bold>t\<^bold>h P2 \<^bold>d\<^bold>u\<^bold>a\<^bold>l h2\<^sub>m \<tycolon> \<medium_left_bracket> H2\<^sub>m \<medium_right_bracket> \<longmapsto> h1\<^sub>m \<tycolon> H1\<^sub>m \<^bold>w\<^bold>h\<^bold>e\<^bold>n Q2
+    \<Longrightarrow> \<^bold>c\<^bold>a\<^bold>s\<^bold>t h \<tycolon> H \<longmapsto> (x, h2) \<tycolon> \<medium_left_bracket> X <heap-sep> H2 \<medium_right_bracket> \<^bold>w\<^bold>i\<^bold>t\<^bold>h P1 \<and> P2 \<^bold>d\<^bold>u\<^bold>a\<^bold>l (x\<^sub>m, h2\<^sub>m) \<tycolon> \<medium_left_bracket> X\<^sub>m <heap-sep> H2\<^sub>m \<medium_right_bracket> \<longmapsto> h\<^sub>m \<tycolon> H\<^sub>m \<^bold>w\<^bold>h\<^bold>e\<^bold>n Q1 \<and> Q2"
+  unfolding Cast_def CastDual_def Heap_Cast_Goal_def SepNu_2_SepSet
+  by (smt (verit, del_insts) SeparationSet_assoc SeparationSet_comm SeparationSet_def mem_Collect_eq)
 
 (* TODO: implement the Different tactic and then enable the \<nu>intro' *)
-lemma [ \<nu>intro' ]: "\<^bold>d\<^bold>e\<^bold>s\<^bold>t \<^bold>c\<^bold>a\<^bold>s\<^bold>t x \<tycolon> T \<longmapsto> D \<^bold>w\<^bold>i\<^bold>t\<^bold>h P \<^bold>w\<^bold>h\<^bold>e\<^bold>n P' \<Longrightarrow> Different \<tort_lbrace> x \<tycolon> T \<tort_rbrace> D \<Longrightarrow> \<^bold>p\<^bold>r\<^bold>e\<^bold>m\<^bold>i\<^bold>s\<^bold>e P'
-  \<Longrightarrow> \<^bold>c\<^bold>a\<^bold>s\<^bold>t D \<longmapsto> D' \<heavy_asterisk> \<medium_left_bracket> H \<medium_right_bracket> \<^bold>w\<^bold>i\<^bold>t\<^bold>h P2 \<^bold>d\<^bold>u\<^bold>a\<^bold>l I'\<^sub>m \<heavy_asterisk> \<medium_left_bracket> H\<^sub>m \<medium_right_bracket> \<longmapsto> I \<^bold>w\<^bold>h\<^bold>e\<^bold>n Q2  
-  \<Longrightarrow> \<^bold>i\<^bold>n\<^bold>t\<^bold>r\<^bold>o \<^bold>c\<^bold>a\<^bold>s\<^bold>t I \<longmapsto> x\<^sub>m \<tycolon> T \<^bold>w\<^bold>i\<^bold>t\<^bold>h Q' \<^bold>w\<^bold>h\<^bold>e\<^bold>n Q
-  \<Longrightarrow> \<^bold>c\<^bold>a\<^bold>s\<^bold>t x \<tycolon> T \<longmapsto> D' \<heavy_asterisk> \<medium_left_bracket> H \<medium_right_bracket> \<^bold>w\<^bold>i\<^bold>t\<^bold>h P \<and> P2 \<^bold>d\<^bold>u\<^bold>a\<^bold>l I'\<^sub>m \<heavy_asterisk> \<medium_left_bracket> H\<^sub>m \<medium_right_bracket> \<longmapsto> x\<^sub>m \<tycolon> T \<^bold>w\<^bold>h\<^bold>e\<^bold>n Q \<and> Q2"
+lemma [ \<nu>intro' ]: "\<^bold>d\<^bold>e\<^bold>s\<^bold>t \<^bold>c\<^bold>a\<^bold>s\<^bold>t x \<tycolon> T \<longmapsto> d \<tycolon> D \<^bold>w\<^bold>i\<^bold>t\<^bold>h P \<^bold>w\<^bold>h\<^bold>e\<^bold>n P' \<Longrightarrow> Different (x \<tycolon> T) (d \<tycolon> D) \<Longrightarrow> \<^bold>p\<^bold>r\<^bold>e\<^bold>m\<^bold>i\<^bold>s\<^bold>e P'
+  \<Longrightarrow> \<^bold>c\<^bold>a\<^bold>s\<^bold>t d \<tycolon> D \<longmapsto> d' \<tycolon> D' \<heavy_asterisk> h \<tycolon> \<medium_left_bracket> H \<medium_right_bracket> \<^bold>w\<^bold>i\<^bold>t\<^bold>h P2 \<^bold>d\<^bold>u\<^bold>a\<^bold>l i'\<^sub>m \<tycolon> I'\<^sub>m \<heavy_asterisk> h\<^sub>m \<tycolon> \<medium_left_bracket> H\<^sub>m \<medium_right_bracket> \<longmapsto> i \<tycolon> I \<^bold>w\<^bold>h\<^bold>e\<^bold>n Q2  
+  \<Longrightarrow> \<^bold>i\<^bold>n\<^bold>t\<^bold>r\<^bold>o \<^bold>c\<^bold>a\<^bold>s\<^bold>t i \<tycolon> I \<longmapsto> x\<^sub>m \<tycolon> T \<^bold>w\<^bold>i\<^bold>t\<^bold>h Q' \<^bold>w\<^bold>h\<^bold>e\<^bold>n Q
+  \<Longrightarrow> \<^bold>c\<^bold>a\<^bold>s\<^bold>t x \<tycolon> T \<longmapsto> d' \<tycolon> D' \<heavy_asterisk> h \<tycolon> \<medium_left_bracket> H \<medium_right_bracket> \<^bold>w\<^bold>i\<^bold>t\<^bold>h P \<and> P2 \<^bold>d\<^bold>u\<^bold>a\<^bold>l i'\<^sub>m \<tycolon> I'\<^sub>m \<heavy_asterisk> h\<^sub>m \<tycolon> \<medium_left_bracket> H\<^sub>m \<medium_right_bracket> \<longmapsto> x\<^sub>m \<tycolon> T \<^bold>w\<^bold>h\<^bold>e\<^bold>n Q \<and> Q2"
   unfolding Dest_def Intro_def CastDual_def Different_def Heap_Cast_Goal_def Cast_def
   by (auto simp add: Premise_def)
 
 
 
-lemma heap_put_this: "\<^bold>c\<^bold>a\<^bold>s\<^bold>t Nothing \<heavy_asterisk> X \<longmapsto> X" unfolding Cast_def Separation_emptyL by simp
-lemma "\<^bold>c\<^bold>a\<^bold>s\<^bold>t S \<heavy_asterisk> X \<longmapsto> S' \<Longrightarrow> \<^bold>c\<^bold>a\<^bold>s\<^bold>t L \<heavy_asterisk> S \<heavy_asterisk> X \<longmapsto> L \<heavy_asterisk> S' "
-  unfolding Cast_def by (smt (verit, del_insts) Separation_assoc Separation_comm Separation_def mem_Collect_eq)
-lemma "\<^bold>c\<^bold>a\<^bold>s\<^bold>t S \<heavy_asterisk> X \<longmapsto> S' \<Longrightarrow> \<^bold>c\<^bold>a\<^bold>s\<^bold>t (S \<heavy_asterisk> R) \<heavy_asterisk> X \<longmapsto> S' \<heavy_asterisk> R "
-  unfolding Cast_def by (smt (verit, del_insts) Separation_assoc Separation_comm Separation_def mem_Collect_eq)
+lemma heap_put_this: "\<^bold>c\<^bold>a\<^bold>s\<^bold>t Nothing \<heavy_asterisk> x \<tycolon> X \<longmapsto> x \<tycolon> X" unfolding Cast_def Separation_emptyL by simp
+lemma "\<^bold>c\<^bold>a\<^bold>s\<^bold>t s \<tycolon> S \<heavy_asterisk> x \<tycolon> X \<longmapsto> s' \<tycolon> S' \<Longrightarrow> \<^bold>c\<^bold>a\<^bold>s\<^bold>t l \<tycolon> L \<heavy_asterisk> s \<tycolon> S \<heavy_asterisk> x \<tycolon> X \<longmapsto> l \<tycolon> L \<heavy_asterisk> s' \<tycolon> S' "
+  unfolding Cast_def SepNu_2_SepSet
+  by (smt (verit, del_insts) SeparationSet_assoc SeparationSet_comm SeparationSet_def mem_Collect_eq)
+lemma "\<^bold>c\<^bold>a\<^bold>s\<^bold>t s \<tycolon> S \<heavy_asterisk> x \<tycolon> X \<longmapsto> s' \<tycolon> S' \<Longrightarrow> \<^bold>c\<^bold>a\<^bold>s\<^bold>t (s \<tycolon> S \<heavy_asterisk> r \<tycolon> R) \<heavy_asterisk> x \<tycolon> X \<longmapsto> s' \<tycolon> S' \<heavy_asterisk> r \<tycolon> R "
+  unfolding Cast_def SepNu_2_SepSet
+  by (smt (verit, del_insts) SeparationSet_assoc SeparationSet_comm SeparationSet_def mem_Collect_eq)
 
 
 
-lemma "\<^bold>c\<^bold>a\<^bold>s\<^bold>t S \<longmapsto> S' \<Longrightarrow> \<^bold>c\<^bold>a\<^bold>s\<^bold>t L \<heavy_asterisk> S \<longmapsto> L \<heavy_asterisk> S'"
-  unfolding Cast_def by (smt (verit, del_insts) Separation_assoc Separation_comm Separation_def mem_Collect_eq) 
+(* lemma "\<^bold>c\<^bold>a\<^bold>s\<^bold>t S \<longmapsto> S' \<Longrightarrow> \<^bold>c\<^bold>a\<^bold>s\<^bold>t L \<heavy_asterisk> S \<longmapsto> L \<heavy_asterisk> S'"
+  unfolding Cast_def by (smt (verit, del_insts) Separation_assoc Separation_comm Separation_def mem_Collect_eq
 lemma "\<^bold>c\<^bold>a\<^bold>s\<^bold>t S \<longmapsto> S' \<Longrightarrow> \<^bold>c\<^bold>a\<^bold>s\<^bold>t S \<heavy_asterisk> R \<longmapsto> S' \<heavy_asterisk> R"
-  unfolding Cast_def by (smt (verit, del_insts) Separation_assoc Separation_comm Separation_def mem_Collect_eq)
+  unfolding Cast_def by (smt (verit, del_insts) Separation_assoc Separation_comm Separation_def mem_Collect_eq *)
 
 
 
@@ -475,8 +524,9 @@ lemma StackDelimiter_to_AndTy: " (A\<heavy_comma> B) \<equiv> (B \<^bold>a\<^bol
 
 subsection \<open>Cast\<close>
 
-theorem apply_cast: "(\<^bold>c\<^bold>u\<^bold>r\<^bold>r\<^bold>e\<^bold>n\<^bold>t blk \<^bold>r\<^bold>e\<^bold>s\<^bold>u\<^bold>l\<^bold>t\<^bold>s \<^bold>i\<^bold>n (R \<heavy_comma> X\<heavy_comma> \<^bold>h\<^bold>e\<^bold>a\<^bold>p H)) \<Longrightarrow> (\<^bold>c\<^bold>a\<^bold>s\<^bold>t X \<longmapsto> Y \<^bold>w\<^bold>i\<^bold>t\<^bold>h P) \<Longrightarrow> (\<^bold>c\<^bold>u\<^bold>r\<^bold>r\<^bold>e\<^bold>n\<^bold>t blk \<^bold>r\<^bold>e\<^bold>s\<^bold>u\<^bold>l\<^bold>t\<^bold>s \<^bold>i\<^bold>n (R \<heavy_comma> Y\<heavy_comma> \<^bold>h\<^bold>e\<^bold>a\<^bold>p H) \<addition> P)"
-  unfolding Procedure_def CurrentConstruction_def PendingConstruction_def bind_def SpecTop_imp Cast_def by (auto 4 6)
+
+theorem apply_cast: "(\<^bold>c\<^bold>u\<^bold>r\<^bold>r\<^bold>e\<^bold>n\<^bold>t blk \<^bold>r\<^bold>e\<^bold>s\<^bold>u\<^bold>l\<^bold>t\<^bold>s \<^bold>i\<^bold>n (R \<heavy_comma> x \<tycolon> X\<heavy_comma> \<^bold>h\<^bold>e\<^bold>a\<^bold>p H)) \<Longrightarrow> (\<^bold>c\<^bold>a\<^bold>s\<^bold>t x \<tycolon> X \<longmapsto> y \<tycolon> Y \<^bold>w\<^bold>i\<^bold>t\<^bold>h P) \<Longrightarrow> (\<^bold>c\<^bold>u\<^bold>r\<^bold>r\<^bold>e\<^bold>n\<^bold>t blk \<^bold>r\<^bold>e\<^bold>s\<^bold>u\<^bold>l\<^bold>t\<^bold>s \<^bold>i\<^bold>n (R \<heavy_comma> y \<tycolon> Y\<heavy_comma> \<^bold>h\<^bold>e\<^bold>a\<^bold>p H) \<and> P)"
+  unfolding Procedure_def CurrentConstruction_def PendingConstruction_def bind_def SpecTop_imp Cast_def by (auto 4 6) 
 theorem "cast": "\<^bold>c\<^bold>u\<^bold>r\<^bold>r\<^bold>e\<^bold>n\<^bold>t blk \<^bold>r\<^bold>e\<^bold>s\<^bold>u\<^bold>l\<^bold>t\<^bold>s \<^bold>i\<^bold>n T \<Longrightarrow> \<^bold>c\<^bold>a\<^bold>s\<^bold>t T \<longmapsto> T' \<^bold>w\<^bold>i\<^bold>t\<^bold>h P \<^bold>w\<^bold>h\<^bold>e\<^bold>n Q \<Longrightarrow> \<^bold>p\<^bold>r\<^bold>e\<^bold>m\<^bold>i\<^bold>s\<^bold>e Q \<Longrightarrow> \<^bold>c\<^bold>u\<^bold>r\<^bold>r\<^bold>e\<^bold>n\<^bold>t blk \<^bold>r\<^bold>e\<^bold>s\<^bold>u\<^bold>l\<^bold>t\<^bold>s \<^bold>i\<^bold>n T' "
   for T' :: "(heap \<times> 'a::lrep) set" unfolding Cast_def CurrentConstruction_def by auto
 
@@ -531,12 +581,14 @@ definition AutoConstruct :: " 'exp \<Rightarrow> ('a::lrep \<longmapsto> 'b::lre
 lemma AutoConstruct: "(\<^bold>c\<^bold>u\<^bold>r\<^bold>r\<^bold>e\<^bold>n\<^bold>t blk \<^bold>r\<^bold>e\<^bold>s\<^bold>u\<^bold>l\<^bold>t\<^bold>s \<^bold>i\<^bold>n S) \<Longrightarrow> AutoConstruct exp f S T \<Longrightarrow> (\<^bold>p\<^bold>e\<^bold>n\<^bold>d\<^bold>i\<^bold>n\<^bold>g f \<^bold>o\<^bold>n blk \<^bold>r\<^bold>e\<^bold>s\<^bold>u\<^bold>l\<^bold>t\<^bold>s \<^bold>i\<^bold>n T)" for exp :: "'exp"
   unfolding AutoConstruct_def using apply_proc .
 
+translations "CONST AutoConstruct exp f (s \<tycolon> S) T" \<rightleftharpoons> "CONST AutoConstruct exp f \<tort_lbrace>s \<tycolon> S\<tort_rbrace> T"
+  "CONST AutoConstruct exp f S (t \<tycolon> T)" \<rightleftharpoons> "CONST AutoConstruct exp f S \<tort_lbrace>t \<tycolon> T\<tort_rbrace>"
+
 (* lemma [simp]: "(Inhabited A \<and> Inhabited B) \<or> (Inhabited A' \<and> Inhabited B')
   \<Longrightarrow> (A\<heavy_comma>B) = (A'\<heavy_comma>B') \<longleftrightarrow> A = A' \<and> B = B'" unfolding Stack_Delimiter_def Inhabited_def by (auto simp add: times_eq_iff) 
 lemma  [elim]: "(A\<heavy_comma>B) = (A'\<heavy_comma>B') \<Longrightarrow> (A = {} \<or> B = {} \<Longrightarrow> A' = {} \<or> B' = {} \<Longrightarrow> C) \<Longrightarrow> (A = A' \<Longrightarrow> B = B' \<Longrightarrow> C) \<Longrightarrow> C"
   unfolding Stack_Delimiter_def by (auto simp add: times_eq_iff)
 *)
-
 
 
 subsection \<open>Index for Shallow Representation\<close>
@@ -565,6 +617,14 @@ definition AdrMap :: " ('a,'b,'x,'y) index \<Rightarrow> 'x set \<Rightarrow> 'a
     (\<forall>f. (\<forall>a. a \<in> X \<longrightarrow> f a \<in> Y) \<longrightarrow> (\<forall>a. a \<in> A \<longrightarrow> map_idx idx f  a \<in> B))"
 declare Map_def[\<nu>index_def]
 
+translations "\<^bold>i\<^bold>n\<^bold>d\<^bold>e\<^bold>x idx \<blangle> x \<tycolon> X \<^bold>@ A \<brangle>" \<rightleftharpoons> "\<^bold>i\<^bold>n\<^bold>d\<^bold>e\<^bold>x idx \<blangle> \<tort_lbrace>x \<tycolon> X\<tort_rbrace> \<^bold>@ A \<brangle>"
+  "\<^bold>i\<^bold>n\<^bold>d\<^bold>e\<^bold>x idx \<blangle> X \<^bold>@ a \<tycolon> A \<brangle>" \<rightleftharpoons> "\<^bold>i\<^bold>n\<^bold>d\<^bold>e\<^bold>x idx \<blangle> X \<^bold>@ \<tort_lbrace> a \<tycolon> A\<tort_rbrace> \<brangle>"
+  "\<^bold>i\<^bold>n\<^bold>d\<^bold>e\<^bold>x idx \<blangle> X \<^bold>@ a \<tycolon> A \<longmapsto> Y \<^bold>@ B \<brangle>" \<rightleftharpoons> "\<^bold>i\<^bold>n\<^bold>d\<^bold>e\<^bold>x idx \<blangle> X \<^bold>@ \<tort_lbrace> a \<tycolon> A\<tort_rbrace>  \<longmapsto> Y \<^bold>@ B \<brangle>"
+  "\<^bold>i\<^bold>n\<^bold>d\<^bold>e\<^bold>x idx \<blangle> x \<tycolon> X \<^bold>@ A \<longmapsto> Y \<^bold>@ B \<brangle>" \<rightleftharpoons> "\<^bold>i\<^bold>n\<^bold>d\<^bold>e\<^bold>x idx \<blangle> \<tort_lbrace>x \<tycolon> X\<tort_rbrace> \<^bold>@ A  \<longmapsto> Y \<^bold>@ B \<brangle>"
+  "\<^bold>i\<^bold>n\<^bold>d\<^bold>e\<^bold>x idx \<blangle> X \<^bold>@ A \<longmapsto> y \<tycolon> Y \<^bold>@ B \<brangle>" \<rightleftharpoons> "\<^bold>i\<^bold>n\<^bold>d\<^bold>e\<^bold>x idx \<blangle> X \<^bold>@ A  \<longmapsto> \<tort_lbrace>y \<tycolon> Y\<tort_rbrace> \<^bold>@ B \<brangle>"
+  "\<^bold>i\<^bold>n\<^bold>d\<^bold>e\<^bold>x idx \<blangle> X \<^bold>@ A \<longmapsto> Y \<^bold>@ b \<tycolon> B \<brangle>" \<rightleftharpoons> "\<^bold>i\<^bold>n\<^bold>d\<^bold>e\<^bold>x idx \<blangle> X \<^bold>@ A  \<longmapsto> Y \<^bold>@ \<tort_lbrace>b  \<tycolon> B\<tort_rbrace> \<brangle>"
+
+
 lemma index_here_getter[\<nu>intro]: "\<^bold>i\<^bold>n\<^bold>d\<^bold>e\<^bold>x index_here \<blangle> A \<^bold>@ A \<brangle>"
   unfolding \<nu>index_def  index_here_def by auto
 lemma index_here_mapper[\<nu>intro]: "\<^bold>i\<^bold>n\<^bold>d\<^bold>e\<^bold>x index_here \<blangle> A \<^bold>@ A \<longmapsto> B \<^bold>@ B \<brangle>"
@@ -573,7 +633,7 @@ lemma index_here_mapper[\<nu>intro]: "\<^bold>i\<^bold>n\<^bold>d\<^bold>e\<^bol
   unfolding \<nu>index_def index_left_def by (cases f) auto
 lemma index_right_getter[\<nu>intro]: "\<^bold>i\<^bold>n\<^bold>d\<^bold>e\<^bold>x f \<blangle> X \<^bold>@ A \<brangle> \<Longrightarrow> \<^bold>i\<^bold>n\<^bold>d\<^bold>e\<^bold>x index_right f \<blangle> X \<^bold>@ (L \<^bold>a\<^bold>n\<^bold>d A) \<brangle>"
   unfolding \<nu>index_def index_right_def by (cases f) auto *)
-lemma index_stack_getter[\<nu>intro]: "\<^bold>i\<^bold>n\<^bold>d\<^bold>e\<^bold>x f \<blangle> X \<^bold>@ A \<brangle> \<Longrightarrow> \<^bold>i\<^bold>n\<^bold>d\<^bold>e\<^bold>x index_right f \<blangle> X \<^bold>@ (A\<heavy_comma> N) \<brangle>"
+lemma index_stack_getter[\<nu>intro]: "\<^bold>i\<^bold>n\<^bold>d\<^bold>e\<^bold>x f \<blangle> X \<^bold>@ a \<tycolon> A \<brangle> \<Longrightarrow> \<^bold>i\<^bold>n\<^bold>d\<^bold>e\<^bold>x index_right f \<blangle> X \<^bold>@ (a \<tycolon> A\<heavy_comma> x \<tycolon> N) \<brangle>"
   unfolding \<nu>index_def index_right_def by (cases f) auto
 (* lemma index_left_mapper[\<nu>intro]:
     "\<^bold>i\<^bold>n\<^bold>d\<^bold>e\<^bold>x f \<blangle> X \<^bold>@ A \<longmapsto> Y \<^bold>@ B\<brangle> \<Longrightarrow> \<^bold>i\<^bold>n\<^bold>d\<^bold>e\<^bold>x index_left f \<blangle> X \<^bold>@ (A \<^bold>a\<^bold>n\<^bold>d R) \<longmapsto> Y \<^bold>@ (B \<^bold>a\<^bold>n\<^bold>d R) \<brangle>"
@@ -582,7 +642,7 @@ lemma index_right_mapper[\<nu>intro]:
     "\<^bold>i\<^bold>n\<^bold>d\<^bold>e\<^bold>x f \<blangle> X \<^bold>@ A \<longmapsto> Y \<^bold>@ B\<brangle> \<Longrightarrow> \<^bold>i\<^bold>n\<^bold>d\<^bold>e\<^bold>x index_right f \<blangle> X \<^bold>@ (L \<^bold>a\<^bold>n\<^bold>d A) \<longmapsto> Y \<^bold>@ (L \<^bold>a\<^bold>n\<^bold>d B) \<brangle>"
   unfolding \<nu>index_def index_right_def by (cases f) auto *)
 lemma index_stack_mapper[\<nu>intro]:
-    "\<^bold>i\<^bold>n\<^bold>d\<^bold>e\<^bold>x f \<blangle> X \<^bold>@ A \<longmapsto> Y \<^bold>@ B\<brangle> \<Longrightarrow> \<^bold>i\<^bold>n\<^bold>d\<^bold>e\<^bold>x index_right f \<blangle> X \<^bold>@ (A\<heavy_comma> N) \<longmapsto> Y \<^bold>@ (B\<heavy_comma> N) \<brangle>"
+    "\<^bold>i\<^bold>n\<^bold>d\<^bold>e\<^bold>x f \<blangle> X \<^bold>@ a \<tycolon> A \<longmapsto> Y \<^bold>@ b \<tycolon> B\<brangle> \<Longrightarrow> \<^bold>i\<^bold>n\<^bold>d\<^bold>e\<^bold>x index_right f \<blangle> X \<^bold>@ (a \<tycolon> A\<heavy_comma> N) \<longmapsto> Y \<^bold>@ (b \<tycolon> B\<heavy_comma> N) \<brangle>"
   unfolding \<nu>index_def index_right_def by (cases f) auto
 
 (*
@@ -706,11 +766,11 @@ translations "P" <= "CONST AndFact P (CONST NoFact)"
 *)
 section \<open>Main implementation of the system\<close>
 
-ML_file_debug NuHelp.ML
 ML_file "./general/binary_tree.ML"
 ML_file "./general/auto_level.ML"
 (* ML_file "./library/path.ML" *)
-ML_file_debug NuBasics.ML
+ML \<open>Syntax.parse_term @{context} "xxx"\<close>
+ML_file NuBasics.ML
 ML_file "./library/general.ML"
 ML_file "./library/instructions.ML"
 ML_file "./general/parser.ML"
@@ -720,7 +780,7 @@ ML_file "./library/exty.ML"
 ML_file NuSys.ML
 (* ML_file "./library/registers.ML" *)
 ML_file "./library/processors.ML"
-ML_file "./library/obtain.ML"
+(* ML_file "./library/obtain.ML" *)
 ML_file NuToplevel.ML 
 
 section \<open>Attributes and Commands\<close>
@@ -756,25 +816,25 @@ val requires_statement = Scan.optional (Parse.$$$ "requires" |-- Parse.!!! state
 val requires_opt1 = Scan.option (Parse.$$$ "requires" |-- Parse.term);
 val _ =
   Outer_Syntax.local_theory_to_proof' \<^command_keyword>\<open>proc\<close> "begin a procedure construction"
-    ((Parse_Spec.opt_thm_name ":" -- Parse.term -- Parse.for_fixes -- Scan.optional Parse_Spec.includes []
+    ((Parse_Spec.opt_thm_name ":" -- Parse.term --| $$$ "\<longmapsto>" -- Parse.term -- Parse.for_fixes -- Scan.optional Parse_Spec.includes []
             -- requires_statement) >>
-        (fn ((((b,arg_ret),fixes),includes),preconds) =>  
-            (begin_proc_cmd false b arg_ret fixes includes preconds)));
+        (fn (((((b,arg),ret),fixes),includes),preconds) =>  
+            (begin_proc_cmd false b arg ret fixes includes preconds)));
 
 val _ =
   Outer_Syntax.local_theory_to_proof' \<^command_keyword>\<open>proc'\<close> "begin a procedure construction"
-    ((Parse_Spec.opt_thm_name ":" -- Parse.term -- Parse.for_fixes -- Scan.optional Parse_Spec.includes []
+    ((Parse_Spec.opt_thm_name ":" -- Parse.term --| $$$ "\<longmapsto>" -- Parse.term -- Parse.for_fixes -- Scan.optional Parse_Spec.includes []
             -- requires_statement) >>
-        (fn ((((b,arg_ret),fixes),includes),preconds) =>  
-            (begin_proc_cmd true b arg_ret fixes includes preconds)));
+        (fn (((((b,arg),ret),fixes),includes),preconds) =>  
+            (begin_proc_cmd true b arg ret fixes includes preconds)));
 
-val loop_variables = $$$ "var" |-- !!! vars;
+(* val loop_variables = $$$ "var" |-- !!! vars;
 val _ =
   Outer_Syntax.local_theory_to_proof' \<^command_keyword>\<open>rec_proc\<close> "begin a recursive procedure construction"
     ((Parse_Spec.opt_thm_name ":" -- Parse.term -- loop_variables -- Parse.for_fixes -- Scan.optional Parse_Spec.includes []
             -- requires_opt1) >>
         (fn (((((b,arg_ret),lvars),fixes),includes),preconds) =>  
-            (begin_rec_proc_cmd b arg_ret lvars fixes includes preconds)));
+            (begin_rec_proc_cmd b arg_ret lvars fixes includes preconds))); *)
 
 val _ =
   Outer_Syntax.command \<^command_keyword>\<open>finish\<close> "Finish the procedure construction"
@@ -810,10 +870,10 @@ val _ =
     (and_list1 ((binding -- opt_attribs -- opt_attribs --| $$$ ":") -- and_list1 (prop -- repeat prop)) >>
       (Toplevel.proof' o (snd ooo NuToplevel.have_aux_cmd)))
 
-val _ =
+(* val _ =
   Outer_Syntax.command \<^command_keyword>\<open>\<nu>obtain\<close> "generalized elimination"
     (Parse.parbinding -- Scan.optional (Parse.vars --| Parse.where_) [] -- structured_statement
-      >> (fn ((a, b), (c, d, e)) => Toplevel.proof' (NuObtain.obtain_cmd a b c d e)));
+      >> (fn ((a, b), (c, d, e)) => Toplevel.proof' (NuObtain.obtain_cmd a b c d e))); 
 
 val _ =
   Outer_Syntax.command \<^command_keyword>\<open>\<nu>choose\<close> "existential elimination"
@@ -822,12 +882,12 @@ val _ =
 
 val _ =
   Outer_Syntax.command \<^command_keyword>\<open>\<nu>choose2\<close> "existential elimination"
-    ( Scan.repeat1 Parse.binding >> (Toplevel.proof o NuObtain.chooseV));
+    ( Scan.repeat1 Parse.binding >> (Toplevel.proof o NuObtain.chooseV)); 
 
 
 val _ =
   Outer_Syntax.command \<^command_keyword>\<open>\<nu>choose_quick\<close> "existential elimination"
-    ( Scan.succeed (Toplevel.proof (NuObtain.obtain_quick_pairs)));
+    ( Scan.succeed (Toplevel.proof (NuObtain.obtain_quick_pairs))); *)
 
 val _ =
   Outer_Syntax.command \<^command_keyword>\<open>\<medium_left_bracket>\<close> "construct nested sub-procedure"
@@ -904,7 +964,7 @@ subsubsection \<open>Essential functions\<close>
 
 \<nu>processor accept_proc 300 \<open>\<^bold>p\<^bold>e\<^bold>n\<^bold>d\<^bold>i\<^bold>n\<^bold>g f \<^bold>o\<^bold>n blk \<^bold>r\<^bold>e\<^bold>s\<^bold>u\<^bold>l\<^bold>t\<^bold>s \<^bold>i\<^bold>n T\<close> \<open>fn ctx => fn th => Scan.succeed (fn _ => NuSys.accept_proc ctx th)\<close>
 
-\<nu>processor move_fact 50 \<open>(\<^bold>c\<^bold>u\<^bold>r\<^bold>r\<^bold>e\<^bold>n\<^bold>t blk \<^bold>r\<^bold>e\<^bold>s\<^bold>u\<^bold>l\<^bold>t\<^bold>s \<^bold>i\<^bold>n T \<addition> P)\<close> \<open>fn ctx => fn meta => Scan.succeed (fn _ =>
+\<nu>processor move_fact 50 \<open>(\<^bold>c\<^bold>u\<^bold>r\<^bold>r\<^bold>e\<^bold>n\<^bold>t blk \<^bold>r\<^bold>e\<^bold>s\<^bold>u\<^bold>l\<^bold>t\<^bold>s \<^bold>i\<^bold>n (x \<tycolon> T) \<and> P)\<close> \<open>fn ctx => fn meta => Scan.succeed (fn _ =>
   meta RS @{thm move_fact_to_star1} handle THM _ => meta RS @{thm move_fact_to_star2})\<close>
 
 \<nu>processor call 9000 \<open>\<^bold>c\<^bold>u\<^bold>r\<^bold>r\<^bold>e\<^bold>n\<^bold>t blk \<^bold>r\<^bold>e\<^bold>s\<^bold>u\<^bold>l\<^bold>t\<^bold>s \<^bold>i\<^bold>n T\<close> \<open> fn ctx => fn meta => NuProcedure.parser >> (fn binding => fn _ =>
@@ -948,9 +1008,9 @@ val ctx = NuSys.load_specthm meta ctx
 \<nu>processor set_\<nu>current 100 \<open>\<^bold>c\<^bold>u\<^bold>r\<^bold>r\<^bold>e\<^bold>n\<^bold>t blk \<^bold>r\<^bold>e\<^bold>s\<^bold>u\<^bold>l\<^bold>t\<^bold>s \<^bold>i\<^bold>n T\<close> \<open>fn ctx => fn meta => Scan.succeed (fn _ =>
   raise Bypass (SOME (meta RS @{thm set_\<nu>current})))\<close>
 
-\<nu>processor choose_AutoExTy 10 \<open>\<^bold>c\<^bold>u\<^bold>r\<^bold>r\<^bold>e\<^bold>n\<^bold>t blk \<^bold>r\<^bold>e\<^bold>s\<^bold>u\<^bold>l\<^bold>t\<^bold>s \<^bold>i\<^bold>n AutoExTyp T\<close> \<open>fn ctx => fn meta =>
+(* \<nu>processor choose_AutoExTy 10 \<open>\<^bold>c\<^bold>u\<^bold>r\<^bold>r\<^bold>e\<^bold>n\<^bold>t blk \<^bold>r\<^bold>e\<^bold>s\<^bold>u\<^bold>l\<^bold>t\<^bold>s \<^bold>i\<^bold>n AutoExTyp T\<close> \<open>fn ctx => fn meta =>
   Parse.list1 Parse.binding >> (fn vars => fn () =>
-    raise Process_State_Call' (meta, NuObtain.chooseV vars))\<close>
+    raise Process_State_Call' (meta, NuObtain.chooseV vars))\<close> *)
 
 (* subsubsection \<open>Registers\<close>
 
@@ -987,12 +1047,15 @@ subsubsection \<open>Literal operations\<close>
 
 \<nu>processor literal_number 9500\<open>\<^bold>c\<^bold>u\<^bold>r\<^bold>r\<^bold>e\<^bold>n\<^bold>t blk \<^bold>r\<^bold>e\<^bold>s\<^bold>u\<^bold>l\<^bold>t\<^bold>s \<^bold>i\<^bold>n T\<close> \<open>fn ctx => fn meta => Parse.number >> (fn num => fn _ =>
   let open NuBasics
-    val term = (stack_of_meta meta |> hd |> dest_RepSet |> dest_nuTy |> #2) handle TERM _ => @{term \<open>\<nat>[32]\<close>}
-    val term = mk_nuTy (Syntax.parse_term ctx num, term) |> Syntax.check_term ctx |> Thm.cterm_of ctx
+    val num = Syntax.parse_term ctx num
+    fun mk term = mk_nuTy (num, term) |> Syntax.check_term ctx |> Thm.cterm_of ctx |> @{print}
+    val term = ((stack_of_meta meta |> hd |> #2 |> mk)
+      handle TERM _ => mk @{term \<open>\<nat>[32]\<close>}
+        | ERROR _ => mk @{term \<open>\<nat>[32]\<close>}) |> @{print}
     val ctx = NuSys.load_specthm meta ctx
   in NuSys.auto_construct ctx term meta  end)
 \<close>
 
-\<nu>cast_overloads E I
+  
 
 end
