NuBasicAbstractors.thy
@@ -53,14 +53,14 @@ lemma [\<nu>intro]: "\<^bold>p\<^bold>r\<^bold>e\<^bold>m\<^bold>i\<^bold>s\<^bo
 lemma "\<nu>Equal (N <where> P) can_eq eq \<longleftrightarrow> \<nu>Equal N (\<lambda>x y. x \<in> P \<and> y \<in> P \<and> can_eq x y) eq"
   unfolding \<nu>Equal_def by auto
 
-definition SchemaCondition (infixl "<where''>" 80) where "SchemaCondition = NuRefine"
+(* definition SchemaCondition (infixl "<where''>" 80) where "SchemaCondition = NuRefine"
 abbreviation WorkingSchemaCondition (infixl "<where''''>" 80) where "WorkingSchemaCondition \<equiv> WorkingProtector SchemaCondition"
 
 lemma [simp]: "\<tort_lbrace>x \<tycolon> N <where'> P\<tort_rbrace> = (\<tort_lbrace>x \<tycolon> N\<tort_rbrace> \<addition> (x \<in> P))" unfolding SchemaCondition_def by auto
 lemma [\<nu>intro]: "\<^bold>c\<^bold>a\<^bold>s\<^bold>t x \<tycolon> N \<longmapsto> y \<tycolon> M <where> P \<^bold>w\<^bold>i\<^bold>t\<^bold>h Q \<Longrightarrow> \<^bold>c\<^bold>a\<^bold>s\<^bold>t x \<tycolon> N \<longmapsto> y \<tycolon> M <where'> P \<^bold>w\<^bold>i\<^bold>t\<^bold>h Q" unfolding SchemaCondition_def . 
 lemma SchemaCondition_simp: "\<tort_lbrace> x \<tycolon> N <where'> P\<tort_rbrace> = \<tort_lbrace> x \<tycolon> N \<^bold>w\<^bold>h\<^bold>e\<^bold>r\<^bold>e P\<tort_rbrace>" unfolding SchemaCondition_def by auto
 lemma refine'_\<nu>cast: "\<^bold>p\<^bold>a\<^bold>r\<^bold>a\<^bold>m P \<Longrightarrow> \<^bold>p\<^bold>r\<^bold>e\<^bold>m\<^bold>i\<^bold>s\<^bold>e x \<in> P \<Longrightarrow> \<^bold>c\<^bold>a\<^bold>s\<^bold>t x \<tycolon> N \<longmapsto> x \<tycolon> (N <where''> P)" unfolding WorkingProtector_def Cast_def by auto
-
+*)
 subsubsection \<open>Down Lifting\<close>
 
 definition DownLift :: "('a, 'b) \<nu> \<Rightarrow> ('c \<Rightarrow> 'b) \<Rightarrow> ('a,'c) \<nu>" (infixl "<down-lift>" 80)
@@ -105,7 +105,7 @@ lemma [\<nu>intro]: "\<^bold>i\<^bold>n\<^bold>t\<^bold>r\<^bold>o \<^bold>c\<^b
 lemma [\<nu>intro]: "(\<And> x.  (g x = y) \<Longrightarrow> \<^bold>d\<^bold>e\<^bold>s\<^bold>t \<^bold>c\<^bold>a\<^bold>s\<^bold>t x \<tycolon> M \<longmapsto> N \<^bold>w\<^bold>i\<^bold>t\<^bold>h P \<^bold>w\<^bold>h\<^bold>e\<^bold>n Q) \<Longrightarrow> \<^bold>d\<^bold>e\<^bold>s\<^bold>t \<^bold>c\<^bold>a\<^bold>s\<^bold>t y \<tycolon> M <up-lift> g \<longmapsto> N \<^bold>w\<^bold>i\<^bold>t\<^bold>h P \<^bold>w\<^bold>h\<^bold>e\<^bold>n Q"
   unfolding Dest_def Cast_def by auto
 
-lemma "\<^bold>d\<^bold>e\<^bold>s\<^bold>t \<^bold>c\<^bold>a\<^bold>s\<^bold>t y \<tycolon> M <up-lift> g \<longmapsto> (\<exists>* x. \<tort_lbrace>x \<tycolon> M\<tort_rbrace> \<addition> (g x = y))"
+lemma "\<^bold>d\<^bold>e\<^bold>s\<^bold>t \<^bold>c\<^bold>a\<^bold>s\<^bold>t y \<tycolon> M <up-lift> g \<longmapsto> (\<exists>* x. x \<tycolon> M \<and>\<^sup>\<nu> (g x = y))"
   unfolding Dest_def Cast_def by auto
 
 lemma "\<^bold>c\<^bold>a\<^bold>s\<^bold>t x \<tycolon> N \<longmapsto> f x \<tycolon> N <up-lift> f" unfolding Cast_def by auto
@@ -184,13 +184,15 @@ lemma [elim,\<nu>elim]: "a \<R_arr_tail> xs \<ratio> Array' N \<Longrightarrow> 
 lemma Array'_to_Ref_\<nu>proc[\<nu>intro]:
  "\<^bold>p\<^bold>r\<^bold>e\<^bold>m\<^bold>i\<^bold>s\<^bold>e i < length xs \<Longrightarrow> \<^bold>p\<^bold>r\<^bold>e\<^bold>m\<^bold>i\<^bold>s\<^bold>e (xs ! i) \<noteq> None \<Longrightarrow>
   \<^bold>d\<^bold>e\<^bold>s\<^bold>t \<^bold>c\<^bold>a\<^bold>s\<^bold>t a \<R_arr_tail> xs \<tycolon> Array' N \<longmapsto> a \<R_arr_tail> xs[i := None] \<tycolon> Array' N \<heavy_asterisk> (a ||+ i) \<R_arr_tail> the (xs ! i) \<tycolon> Ref N"
-  unfolding Dest_def Cast_def apply (cases a) apply auto apply (rule heap_split_by_addr_set[of _  _ "-{a ||+ i}"])
+  unfolding Dest_def Cast_def Heap_Delimiter_def
+  apply (cases a) apply auto apply (rule heap_split_by_addr_set[of _  _ "-{a ||+ i}"])
   by (auto simp add: pred_option_def Ball_def nth_list_update)
 
 lemma [\<nu>intro]:
   "\<^bold>p\<^bold>r\<^bold>e\<^bold>m\<^bold>i\<^bold>s\<^bold>e i < length xs \<Longrightarrow>
   \<^bold>i\<^bold>n\<^bold>t\<^bold>r\<^bold>o \<^bold>c\<^bold>a\<^bold>s\<^bold>t a \<R_arr_tail> xs[i := None] \<tycolon> Array' N \<heavy_asterisk> (a ||+ i) \<R_arr_tail> y \<tycolon> Ref N \<longmapsto> a \<R_arr_tail> xs[i := Some y] \<tycolon> Array' N"
-  unfolding Intro_def Cast_def apply (cases a) apply (auto simp add: pred_option_def Ball_def)
+  unfolding Intro_def Cast_def Heap_Delimiter_def
+  apply (cases a) apply (auto simp add: pred_option_def Ball_def)
   by (metis MemAddrState_add_I1 MemAddrState_add_I2 nth_list_update option.sel)
 
 (* lemma Array'_dual_Ref_\<nu>proc [\<nu>intro]:
