NuHelpMath.thy
@@ -8,6 +8,7 @@ notation pred_prod (infixr "\<times>\<^sub>p" 80)
 
 lemma pair_exists: "Ex P \<longleftrightarrow> (\<exists>a b. P (a,b))" using split_paired_Ex .
 lemma pair_forall: "All P \<longleftrightarrow> (\<forall>a b. P (a,b))" using split_paired_All .
+lemmas pair_All = split_paired_all
 
 lemma conj_imp: "(P \<and> Q \<Longrightarrow> PROP R) \<equiv> (P \<Longrightarrow> Q \<Longrightarrow> PROP R)" by rule simp+
 end
